stack-based proof

src/simple-proof/proof-stacks/Binding.v
@@ -8,46 +8,31 @@
 
 Set Implicit Arguments.
 
-Require Import Coq.Program.Equality List.
 Require Import LibLN.
+Require Import Coq.Program.Equality.
 Require Import Definitions.
 
+(** * Substitution Definitions *)
 
 (** Substitution on variables: [a[u/z]] (substituting [z] with [u] in [a]). *)
-
-Definition subst_var (z: var) (u: var) (x: var): var :=
-  If x = z then u else x.
-
-Definition subst_var_p (z: var) (u: path) (x: var): path :=
-  If x = z then u else (pvar x).
-
-Hint Unfold subst_var subst_var_p.
-
-Definition subst_avar (z: var) (u: path) (a: avar) : path :=
+Definition subst_avar (z: var) (u: var) (a: avar) : avar :=
   match a with
-  | avar_b i => p_sel (avar_b i) nil
-  | avar_f x => subst_var_p z u x
-  end.
-
-(* p    [u / z] where p = x.bs:
-   x.bs [u / z] == x [u / z] . bs *)
-Definition subst_path (z: var) (u: path) (p: path) : path :=
-  match p with
-  | p_sel x bs => sel_fields (subst_avar z u x) bs
+  | avar_b i => avar_b i
+  | avar_f x => (avar_f (If x = z then u else x))
   end.
 
 (** Substitution on types and declarations: [T[u/z]] and [D[u/z]]. *)
-Fixpoint subst_typ (z: var) (u: path) (T: typ) { struct T } : typ :=
+Fixpoint subst_typ (z: var) (u: var) (T: typ) { struct T } : typ :=
   match T with
   | typ_top        => typ_top
   | typ_bot        => typ_bot
   | typ_rcd D      => typ_rcd (subst_dec z u D)
   | typ_and T1 T2  => typ_and (subst_typ z u T1) (subst_typ z u T2)
-  | typ_path q L    => typ_path (subst_path z u q) L
+  | typ_sel x L    => typ_sel (subst_avar z u x) L
   | typ_bnd T      => typ_bnd (subst_typ z u T)
   | typ_all T U    => typ_all (subst_typ z u T) (subst_typ z u U)
   end
-with subst_dec (z: var) (u: path) (D: dec) { struct D } : dec :=
+with subst_dec (z: var) (u: var) (D: dec) { struct D } : dec :=
   match D with
   | dec_typ L T U => dec_typ L (subst_typ z u T) (subst_typ z u U)
   | dec_trm L U => dec_trm L (subst_typ z u U)
@@ -55,37 +40,33 @@ with subst_dec (z: var) (u: path) (D: dec) { struct D } : dec :=
 
 (** Substitution on terms, values, and definitions:
     [t[u/z]], [v[u/z]], [d[u/z]]. *)
-Fixpoint subst_trm (z: var) (u: path) (t: trm) : trm :=
+Fixpoint subst_trm (z: var) (u: var) (t: trm) : trm :=
   match t with
+  | trm_var x        => trm_var (subst_avar z u x)
   | trm_val v        => trm_val (subst_val z u v)
-  | trm_path p       => trm_path (subst_path z u p)
-  | trm_app x1 x2    => trm_app (subst_path z u x1) (subst_path z u x2)
+  | trm_sel x1 L     => trm_sel (subst_avar z u x1) L
+  | trm_app x1 x2    => trm_app (subst_avar z u x1) (subst_avar z u x2)
   | trm_let t1 t2    => trm_let (subst_trm z u t1) (subst_trm z u t2)
   end
-with subst_val (z: var) (u: path) (v: val) : val :=
+with subst_val (z: var) (u: var) (v: val) : val :=
   match v with
   | val_new T ds     => val_new (subst_typ z u T) (subst_defs z u ds)
   | val_lambda T t   => val_lambda (subst_typ z u T) (subst_trm z u t)
   end
-with subst_def (z: var) (u: path) (d: def) : def :=
+with subst_def (z: var) (u: var) (d: def) : def :=
   match d with
   | def_typ L T => def_typ L (subst_typ z u T)
   | def_trm L t => def_trm L (subst_trm z u t)
   end
-with subst_defs (z: var) (u: path) (ds: defs) : defs :=
+with subst_defs (z: var) (u: var) (ds: defs) : defs :=
   match ds with
   | defs_nil => defs_nil
   | defs_cons rest d => defs_cons (subst_defs z u rest) (subst_def z u d)
   end.
 
 (** Substitution on the types of a typing environment: [G[u/z]]. *)
-Definition subst_ctx (z: var) (u: path) (G: ctx) : ctx :=
+Definition subst_ctx (z: var) (u: var) (G: ctx) : ctx :=
   map (subst_typ z u) G.
-
-(** * Lemmas *)
-
-(** The following [subst_fresh_XYZ] lemmas state that if [x] is not free
-    in a symbol [Y], then [Y[z/x] = Y]. *)
 
 (** Substitution on the values of an evaluation context: [e[y/x]]. *)
 Definition subst_env x y e := map (subst_val x y) e.
@@ -93,72 +74,12 @@ Definition subst_env x y e := map (subst_val x y) e.
 
 (** * Opening Lemmas *)
 
-(** * Lemmas About Opening *)
-
-Lemma open_var_path_eq : forall x p n,
-    open_rec_path n x p = open_rec_path_p n (pvar x) p.
-Proof.
-  intros. destruct p, a. simpl. repeat case_if*. rewrite* app_nil_r.
-  simpl. reflexivity.
-Qed.
-
-Lemma open_var_typ_dec_eq: forall x,
-    (forall T : typ, forall n : nat,
-          open_rec_typ n x T = open_rec_typ_p n (pvar x) T) /\
-    (forall D : dec, forall n : nat,
-          open_rec_dec n x D = open_rec_dec_p n (pvar x) D).
-Proof.
-  intros. apply typ_mutind; unfold open_typ, open_typ_p; simpl; intros; auto;
-            try solve [rewrite* H; rewrite* H0].
-  unfold open_rec_avar, open_rec_avar_p. rewrite* open_var_path_eq.
-Qed.
-
-Lemma open_var_typ_eq: forall x T,
-  open_typ x T = open_typ_p (pvar x) T.
-Proof.
-  intros. apply open_var_typ_dec_eq.
-Qed.
-
-Lemma open_var_dec_eq: forall x D,
-  open_dec x D = open_dec_p (pvar x) D.
-Proof.
-  intros. apply open_var_typ_dec_eq.
-Qed.
-
-Hint Rewrite open_var_typ_eq open_var_dec_eq open_var_path_eq.
-
-Lemma open_var_trm_val_def_eq : forall x,
-  (forall t n,
-      open_rec_trm n x t = open_rec_trm_p n (pvar x) t) /\
-  (forall v n,
-      open_rec_val n x v = open_rec_val_p n (pvar x) v) /\
-  (forall d n,
-      open_rec_def n x d = open_rec_def_p n (pvar x) d) /\
-  (forall ds n,
-      open_rec_defs n x ds = open_rec_defs_p n (pvar x) ds).
-Proof.
-  introv. apply trm_mutind; intros; simpl; f_equal*;
-            try (rewrite* open_var_path_eq); rewrite* (proj1 (open_var_typ_dec_eq x)).
-Qed.
-
-Lemma open_var_defs_eq: forall x ds,
-    open_defs x ds = open_defs_p (pvar x) ds.
-Proof.
-  intros. apply* open_var_trm_val_def_eq.
-Qed.
-
-Lemma open_var_trm_eq: forall x t,
-    open_trm x t = open_trm_p (pvar x) t.
-Proof.
-  intros. apply* open_var_trm_val_def_eq.
-Qed.
-
 Ltac avar_solve :=
   repeat match goal with
   | [ a: avar |- _ ] =>
     destruct a; simpl; auto; repeat case_if; subst; simpls; repeat case_if*;
     subst; simpls; repeat case_if*
-         end.
+  end.
 
 (** The following [open_fresh_XYZ_injective] lemmas state that given two
     symbols (variables, types, terms, etc.) [X] and [Y] and a variable [z],
@@ -174,17 +95,37 @@ Proof.
   intros. avar_solve; inversion* H1; try (inversions H3; false* notin_same).
 Qed.
 
+(** - types and declarations *)
+Lemma open_fresh_typ_dec_injective:
+  (forall T T' k x,
+    x \notin fv_typ T ->
+    x \notin fv_typ T' ->
+    open_rec_typ k x T = open_rec_typ k x T' ->
+    T = T') /\
+  (forall D D' k x,
+    x \notin fv_dec D ->
+    x \notin fv_dec D' ->
+    open_rec_dec k x D = open_rec_dec k x D' ->
+    D = D').
+Proof.
+
+  Ltac invert_open :=
+    match goal with
+    | [ H: open_rec_typ _ _ _ = open_rec_typ _ _ ?T' |- _ ] =>
+       destruct T'; inversions* H
+    | [ H: open_rec_dec _ _ _ = open_rec_dec _ _ ?D' |- _ ] =>
+       destruct D'; inversions* H
+    end.
+
+  apply typ_mutind; intros; invert_open; simpl in *;
+    f_equal; eauto using open_fresh_avar_injective.
+Qed.
+
 (** The following [lc_open_rec_open_XYZ] lemmas state that if opening
     a symbol (variables, types, terms, etc.) at index [n] that is
     already opened at index [m] results in the same opened symbol,
     opening the symbol itself at index [n] results in the same symbol. *)
 
-(** - paths *)
-Lemma lc_open_rec_open_path: forall p T n m x,
-    n <> m ->
-    open_rec_path n x (open_rec_path m p T) = open_rec_path m p T ->
-    open_rec_path n x T = T.
-Proof. Admitted.
 
 (** - types and declarations *)
 Lemma lc_open_rec_open_typ_dec: forall x y,
@@ -199,11 +140,10 @@ Lemma lc_open_rec_open_typ_dec: forall x y,
 Proof.
   introv. apply typ_mutind; intros; simpls; auto; avar_solve;
             try solve [(inversions H1; erewrite H; eauto)
-                       || (inversions H2; erewrite H; eauto; erewrite H0; eauto)].
-Admitted. (*
+                      || (inversions H2; erewrite H; eauto; erewrite H0; eauto)].
   - inversions H1. rewrite H with (m:=S m); auto.
   - inversions H2. erewrite H; eauto. rewrite H0 with (m:=S m); auto.
-Qed.*)
+Qed.
 
 (** - terms, values, definitions, and list of definitions *)
 Lemma lc_open_rec_open_trm_val_def_defs: forall x y,
@@ -231,7 +171,7 @@ Proof.
       match goal with
       | [ H : _ = _ |- _ ] => injection H as ?; f_equal; eauto
       end; avar_solve.
-Admitted.
+Qed.
 
 (** [x \notin fv(x, y)] #<br>#
     [―――――――――――――――――] #<br>#
@@ -243,13 +183,6 @@ Proof.
   intros. destruct z; simpls; try case_if; unfold fv_avar; auto.
 Qed.
 
-Lemma open_fv_path : forall x y k p,
-    x \notin fv_path p \u \{y} ->
-    x \notin fv_path (open_rec_path k y p).
-Proof.
-  intros. destruct p; simpls. apply* open_fv_avar.
-Qed.
-
 (** [x \notin fv(T, y)] #<br>#
     [―――――――――――――――――] #<br>#
     [x \notin fv(T^y)] *)
@@ -258,7 +191,7 @@ Lemma open_fv_typ_dec :
   (forall D x y k, x \notin fv_dec D \u \{y} -> x \notin fv_dec (open_rec_dec k y D)).
 Proof.
   apply typ_mutind; intros; simpls; auto;
-    apply open_fv_path; auto.
+    apply open_fv_avar; auto.
 Qed.
 
 (** [x \notin fv(t, y)] #<br>#
@@ -273,8 +206,9 @@ Proof.
   Local Hint Resolve open_fv_avar.
   apply trm_mutind; intros; simpls; auto;
     try apply notin_union_l;
-    try (apply open_fv_typ_dec || apply open_fv_path); auto.
+    try apply open_fv_typ_dec; auto.
 Qed.
+
 
 (** * Local Closure
 
@@ -289,9 +223,6 @@ Inductive lc_at_var (k : nat) : avar -> Prop :=
 | lc_at_b : forall i, i < k -> lc_at_var k (avar_b i).
 Hint Constructors lc_at_var.
 
-Inductive lc_at_path (k: nat) : path -> Prop :=
-| lc_at_p : forall x bs, lc_at_var k x -> lc_at_path k (p_sel x bs).
-Hint Constructors lc_at_path.
 
 (** Locally closed types and declarations. *)
 Inductive lc_at_typ (k : nat) : typ -> Prop :=
@@ -305,8 +236,8 @@ Inductive lc_at_typ (k : nat) : typ -> Prop :=
     lc_at_typ k T2 ->
     lc_at_typ k (typ_and T1 T2)
 | lc_at_typ_sel : forall x L,
-    lc_at_path k x ->
-    lc_at_typ k (typ_path x L)
+    lc_at_var k x ->
+    lc_at_typ k (typ_sel x L)
 | lc_at_typ_bnd : forall T,
     lc_at_typ (S k) T ->
     lc_at_typ k (typ_bnd T)
@@ -327,15 +258,18 @@ Hint Constructors lc_at_typ lc_at_dec.
 
 (** Locally closed terms, values, and definitions. *)
 Inductive lc_at_trm (k : nat) : trm -> Prop :=
-| lc_at_trm_path : forall p,
-    lc_at_path k p ->
-    lc_at_trm k (trm_path p)
+| lc_at_trm_var : forall a,
+    lc_at_var k a ->
+    lc_at_trm k (trm_var a)
 | lc_at_trm_val : forall v,
     lc_at_val k v ->
     lc_at_trm k (trm_val v)
+| lc_at_trm_sel : forall x a,
+    lc_at_var k x ->
+    lc_at_trm k (trm_sel x a)
 | lc_at_trm_app : forall f a,
-    lc_at_path k f ->
-    lc_at_path k a ->
+    lc_at_var k f ->
+    lc_at_var k a ->
     lc_at_trm k (trm_app f a)
 | lc_at_trm_let : forall t1 t2,
     lc_at_trm k t1 ->
@@ -367,7 +301,6 @@ Hint Constructors lc_at_trm lc_at_val lc_at_def lc_at_defs.
 
 
 Notation "'lc_var' x" := (lc_at_var 0 x) (at level 0).
-Notation "'lc_path' p" := (lc_at_path 0 p) (at level 0).
 Notation "'lc_typ' T" := (lc_at_typ 0 T) (at level 0).
 Notation "'lc_dec' D" := (lc_at_dec 0 D) (at level 0).
 
@@ -399,12 +332,6 @@ Hint Constructors lc_ec.
 
 (** ** Local Closure Lemmas *)
 
-Lemma lc_at_relaxing_path : forall k j p,
-    lc_at_path k p -> j >= k -> lc_at_path j p.
-Proof.
-  introv Hl Hjk. inversions Hl. constructor. inversions H; constructor. omega.
-Qed.
-
 Lemma lc_at_relaxing_typ_dec :
     (forall T k j, lc_at_typ k T -> j >= k -> lc_at_typ j T) /\
     (forall D k j, lc_at_dec k D -> j >= k -> lc_at_dec j D).
@@ -421,9 +348,9 @@ Proof with auto.
     try match goal with
         | [ H : _ -> _ |- _ ] => eapply H; try eassumption
         end;
-    try (apply* lc_at_relaxing_path);
     omega.
 Qed.
+
 
 Lemma lc_at_relaxing_trm_val_def_defs:
   (forall t k j, lc_at_trm k t -> j >= k -> lc_at_trm j t) /\
@@ -447,7 +374,6 @@ Proof.
     try match goal with
         | [ H : _ -> _ |- _ ] => eapply H; try eassumption
         end;
-    try (apply* lc_at_relaxing_path);
     omega.
 Qed.
 
@@ -460,11 +386,6 @@ Proof with auto.
   constructor. omega.
 Qed.
 
-Lemma lc_at_to_open_path : forall p k x,
-    lc_at_path (S k) p -> lc_at_path k (open_rec_path k x p).
-Proof.
-  introv Hl. inversions Hl. constructor. apply* lc_at_to_open_avar.
-Qed.
 
 Lemma lc_at_to_open_typ_dec : forall x,
     (forall T k, lc_at_typ (S k) T -> lc_at_typ k (open_rec_typ k x T)) /\
@@ -477,8 +398,9 @@ Proof.
     | [ H : lc_at_dec (S _) _ |- _ ] => inversions H
     end;
     try solve [constructor; try fold open_rec_dec; try fold open_rec_typ; auto];
-    solve [repeat constructor; apply lc_at_to_open_path; auto].
+    solve [repeat constructor; apply lc_at_to_open_avar; auto].
 Qed.
+
 
 Lemma lc_at_to_open_trm_val_def_defs : forall x,
     (forall t k, lc_at_trm (S k) t -> lc_at_trm k (open_rec_trm k x t)) /\
@@ -498,25 +420,20 @@ Proof.
     repeat constructor; auto;
     try solve [try fold open_rec_trm; auto];
     try solve [apply lc_at_to_open_typ_dec; auto];
-    solve [apply lc_at_to_open_path; auto].
+    solve [apply lc_at_to_open_avar; auto].
 Qed.
 
-Lemma open_to_lc_at_avar : forall x y k,
-    lc_at_var k (open_rec_avar k x y) ->
-    lc_at_var (S k) y.
+
+Lemma open_to_lc_at_avar : forall x v k,
+    lc_at_var k (open_rec_avar k x v) ->
+    lc_at_var (S k) v.
 Proof.
   intros. inversion H; subst;
-      destruct y; simpl in *;
+      destruct v; simpl in *;
         try case_if; subst; repeat constructor; auto.
   inversion H0. omega.
 Qed.
 
-Lemma open_to_lc_at_path : forall k x p,
-    lc_at_path k (open_rec_path k x p) ->
-    lc_at_path (S k) p.
-Proof.
-  introv Hl. inversions Hl. destruct p. inversions H. constructor. apply* open_to_lc_at_avar.
-Qed.
 
 Lemma open_to_lc_at_typ_dec : forall x,
     (forall T k, lc_at_typ k (open_rec_typ k x T) -> lc_at_typ (S k) T) /\
@@ -529,8 +446,9 @@ Proof with eauto.
     | [ H : lc_at_dec _ _ |- _ ] => inversions H
     end;
     repeat constructor; auto;
-      eapply open_to_lc_at_path...
+      eapply open_to_lc_at_avar...
 Qed.
+
 
 Lemma open_to_lc_at_trm_val_def_defs : forall x,
     (forall t k, lc_at_trm k (open_rec_trm k x t) -> lc_at_trm (S k) t) /\
@@ -549,21 +467,19 @@ Proof.
     end;
     repeat constructor; auto;
     try solve [try fold open_rec_trm; auto];
-    first [eapply open_to_lc_at_typ_dec | eapply open_to_lc_at_path]; eauto.
+    first [eapply open_to_lc_at_typ_dec | eapply open_to_lc_at_avar]; eauto.
 Qed.
 
 
 Lemma open_left_inverse_close_avar:
-  forall y x k, lc_at_var k y -> open_rec_avar k x (close_rec_avar k x y) = y.
+  forall v x k, lc_at_var k v -> open_rec_avar k x (close_rec_avar k x v) = v.
 Proof with auto.
   intros. unfold open_rec_avar, close_rec_avar.
   inversion H; repeat case_if; subst...
   omega.
 Qed.
 Hint Resolve open_left_inverse_close_avar.
-(*
-Lemma open_left_inverse_close_path:
-  forall p x k, lc_at_path k p -> open_rec_avar k x (close_rec_path k x p) = p.*)
+
 
 Lemma open_left_inverse_close_typ_dec:
   (forall T x k, lc_at_typ k T -> open_rec_typ k x (close_rec_typ k x T) = T) /\
@@ -575,7 +491,8 @@ Proof with auto.
   | [ H : lc_at_dec _ _ |- _ ] => inversions H
   end;
   try apply func_eq_2;
-  try apply func_eq_1... Admitted.
+  try apply func_eq_1...
+Qed.
 
 
 Lemma open_left_inverse_close_trm_val_def_defs :
@@ -583,7 +500,7 @@ Lemma open_left_inverse_close_trm_val_def_defs :
   (forall v k x, lc_at_val k v -> open_rec_val k x (close_rec_val k x v) = v) /\
   (forall d k x, lc_at_def k d -> open_rec_def k x (close_rec_def k x d) = d) /\
   (forall ds k x, lc_at_defs k ds -> open_rec_defs k x (close_rec_defs k x ds) = ds).
-Proof. Admitted. (*
+Proof.
   apply trm_mutind; intros; simpl in *; auto;
     match goal with
     | [ H : lc_at_trm _ _ |- _ ] => inversions H
@@ -594,7 +511,7 @@ Proof. Admitted. (*
     try apply func_eq_2;
     try apply func_eq_1; auto;
       apply open_left_inverse_close_typ_dec; auto.
-Qed.*)
+Qed.
 
 
 (** The following [lc_at_opening_XYZ] lemmas state that opening a locally
@@ -618,11 +535,11 @@ Lemma lc_at_opening_typ_dec: forall x m,
     (forall D, lc_at_dec m D -> forall n, n >= m -> open_rec_dec n x D = D).
 Proof.
   Local Hint Resolve lc_at_opening_avar.
-  intro x. Admitted. (*apply lc_at_typ_mutind; intros; simpls; f_equal*;
+  intro x. apply lc_at_typ_mutind; intros; simpls; f_equal*;
   match goal with
   | [ H : _ -> _ -> open_rec_typ _ _ _ = _ |- _ ] => apply H
   end; omega.
-Qed.*)
+Qed.
 
 
 (** - terms, values, definitions, and list of definitions *)
@@ -633,7 +550,7 @@ Lemma lc_at_opening_trm_val_def_defs: forall x m,
   (forall ds, lc_at_defs m ds -> forall n, n >= m -> open_rec_defs n x ds = ds).
 Proof.
   Local Hint Resolve lc_at_opening_avar.
-  intro x. Admitted. (*
+  intro x.
   apply lc_at_mutind; intros; simpls; f_equal*;
     try solve
         [match goal with
@@ -642,7 +559,7 @@ Proof.
   eapply lc_at_opening_typ_dec;
     try eassumption;
     try omega.
-Qed.*)
+Qed.
 
 
 (** The [lc_at_opening_trm_val_def_defs] lemma, specialized to terms. *)
@@ -718,13 +635,13 @@ Lemma close_rec_typ_dec_no_capture : forall x,
     (forall T k, x \notin fv_typ (close_rec_typ k x T)) /\
     (forall D k, x \notin fv_dec (close_rec_dec k x D)).
 Proof.
-  intros x. Admitted. (*
+  intros x.
   apply typ_mutind; intros; simpl; auto;
     match goal with
     | [ |- _ \notin fv_avar (close_rec_avar _ _ ?a) ] => destruct a
     end; simpl;
       try case_if; unfold fv_avar; auto.
-Qed.*)
+Qed.
 
 (** - for terms, values, and definitions *)
 Lemma close_rec_trm_val_def_defs_no_capture: forall x,
@@ -742,7 +659,8 @@ Proof.
       match goal with
       | [ |- _ \notin fv_avar (close_rec_avar _ _ ?a) ] => destruct a; simpl
       end;
-    repeat case_if; unfold fv_avar; auto. Admitted.
+    repeat case_if; unfold fv_avar; auto.
+Qed.
 
 (** * Free Variables Lemmas *)
 
@@ -797,7 +715,7 @@ Qed.
 (** Substitution preserves local closure. *)
 
 (** - for variables *)
-(*Lemma lc_at_subst_avar : forall v x y k,
+Lemma lc_at_subst_avar : forall v x y k,
     lc_at_var k v <-> lc_at_var k (subst_avar x y v).
 Proof.
   intros.
@@ -805,14 +723,15 @@ Proof.
     try solve [inversion H; simpls; auto].
   destruct v; auto.
 Qed.
-*)
+
 (** - for types and declarations *)
 Lemma lc_at_subst_typ_dec : forall k,
   (forall T, lc_at_typ k T -> forall x y, lc_at_typ k (subst_typ x y T)) /\
   (forall D, lc_at_dec k D -> forall x y, lc_at_dec k (subst_dec x y D)).
 Proof.
   apply lc_at_typ_mutind; intros; simpls; auto.
-  constructor. Admitted. (*apply lc_at_subst_avar. trivial.*)
+  constructor. apply lc_at_subst_avar. trivial.
+Qed.
 
 (** - for terms, values, and definitions *)
 Lemma lc_at_subst_trm_val_def_defs : forall k,
@@ -825,9 +744,7 @@ Proof.
     repeat constructor;
     try solve [apply lc_at_subst_avar; trivial];
     try apply lc_at_subst_typ_dec; trivial.
-Admitted.
-
-(** * Lemmas *)
+Qed.
 
 (** The following [subst_fresh_XYZ] lemmas state that if [x] is not free
     in a symbol [Y], then [Y[z/x] = Y]. *)
@@ -835,32 +752,21 @@ Admitted.
 (** Fresh substitution
     - in variables *)
 Lemma subst_fresh_avar: forall x y,
-  (forall a: avar, x \notin fv_avar a -> subst_avar x y a = p_sel a nil).
+  (forall a: avar, x \notin fv_avar a -> subst_avar x y a = a).
 Proof.
-  intros. destruct* a. simpl. autounfold. case_var*. simpls. notin_false.
+  intros. destruct* a. simpl. case_var*. simpls. notin_false.
 Qed.
 
-Lemma subst_fresh_path : forall x q p,
-    x \notin fv_path p ->
-    subst_path x q p = p.
-Proof.
-  intros. destruct p as [[n | z] bs]; simpls.
-  - Case "p = (avar_b n).bs".
-    rewrite* app_nil_r.
-  - Case "p = (avar_f z).bs".
-    unfold subst_var_p. apply notin_singleton in H. case_if.
-    simpl. rewrite* app_nil_r.
-Qed.
-
-(** - in types, declarations, paths *)
+(** - in types and declarations *)
 Lemma subst_fresh_typ_dec: forall x y,
-  (forall T : typ  , x \notin fv_typ  T  -> subst_typ  x y T  = T ) /\
-  (forall D : dec  , x \notin fv_dec  D  -> subst_dec  x y D  = D ).
+  (forall T : typ , x \notin fv_typ  T  -> subst_typ  x y T  = T ) /\
+  (forall D : dec , x \notin fv_dec  D  -> subst_dec  x y D  = D ).
 Proof.
-  intros x y. apply typ_mutind; intros; simpls; f_equal*. apply* subst_fresh_path.
+  intros x y. apply typ_mutind; intros; simpls; f_equal*.
+  apply* subst_fresh_avar.
 Qed.
 
-Definition subst_fresh_typ x p := proj1 (subst_fresh_typ_dec x p).
+Definition subst_fresh_typ(x y: var) := proj1 (subst_fresh_typ_dec x y).
 
 (** - in terms, values, and definitions *)
 Lemma subst_fresh_trm_val_def_defs: forall x y,
@@ -870,7 +776,222 @@ Lemma subst_fresh_trm_val_def_defs: forall x y,
   (forall ds: defs, x \notin fv_defs ds -> subst_defs x y ds = ds).
 Proof.
   intros x y. apply trm_mutind; intros; simpls; f_equal*;
-    (apply* subst_fresh_typ_dec || apply* subst_fresh_path).
+    (apply* subst_fresh_avar || apply* subst_fresh_typ_dec).
+Qed.
+
+(** [x \notin fv(G, z: T)]                   #<br>#
+    [x \notin fv(T)]                         #<br>#
+    [―――――――――――――――――――――――――――――――――――――] #<br>#
+    [x \notin fv(T)] and [x \notin fv(G)] *)
+Lemma invert_fv_ctx_types_push: forall x z T G,
+  x \notin fv_ctx_types (G & z ~ T) -> x \notin fv_typ T /\ x \notin (fv_ctx_types G).
+Proof.
+  introv H. rewrite fv_ctx_types_push_eq in H.
+  apply~ notin_union.
+Qed.
+
+(** [x \notin fv(G)]         #<br>#
+    [――――――――――――――――――]    #<br>#
+    [G[y/x] = G]    *)
+Lemma subst_fresh_ctx: forall x y G,
+  x \notin fv_ctx_types G -> subst_ctx x y G = G.
+Proof.
+  intros x y.
+  apply (env_ind (fun G => x \notin fv_ctx_types G -> subst_ctx x y G = G)).
+  + intro N. unfold subst_ctx. apply map_empty.
+  + intros G z T IH N.
+    apply invert_fv_ctx_types_push in N. destruct N as [N1 N2].
+    unfold subst_ctx in *. rewrite map_push.
+    rewrite (IH N2).
+    rewrite ((proj1 (subst_fresh_typ_dec _ _)) _ N1).
+    reflexivity.
+Qed.
+
+(** Definition of substitution on named variables: #<br>#
+    [z[y/x] := if z == x then y else z], where [z] is a named variable. *)
+Definition subst_fvar(x y z: var): var := If z = x then y else z.
+
+(** The following lemmas state that substitution commutes with opening:
+    for a symbol [Z], #<br>#
+    [(Z^a)[y/x] = (Z[y/x])^(a[y/x])]. *)
+
+(** Substitution commutes with opening
+    - variables *)
+Lemma subst_open_commut_avar: forall x y u,
+  (forall a: avar, forall n: Datatypes.nat,
+    subst_avar x y (open_rec_avar n u a)
+    = open_rec_avar n (subst_fvar x y u) (subst_avar  x y a)).
+Proof.
+  intros. unfold subst_fvar, subst_avar, open_avar, open_rec_avar. destruct a.
+  + repeat case_if; auto.
+  + case_var*.
+Qed.
+
+(** - types and declarations *)
+Lemma subst_open_commut_typ_dec: forall x y u,
+  (forall t : typ, forall n: nat,
+     subst_typ x y (open_rec_typ n u t)
+     = open_rec_typ n (subst_fvar x y u) (subst_typ x y t)) /\
+  (forall D : dec, forall n: nat,
+     subst_dec x y (open_rec_dec n u D)
+     = open_rec_dec n (subst_fvar x y u) (subst_dec x y D)).
+Proof.
+  intros. apply typ_mutind; intros; simpl; f_equal*.
+  apply subst_open_commut_avar.
+Qed.
+
+(** - types only *)
+Lemma subst_open_commut_typ: forall x y u T,
+  subst_typ x y (open_typ u T) = open_typ (subst_fvar x y u) (subst_typ x y T).
+Proof.
+  intros. apply subst_open_commut_typ_dec.
+Qed.
+
+(** - terms, values, definitions, and list of definitions *)
+Lemma subst_open_commut_trm_val_def_defs: forall x y u,
+  (forall t : trm, forall n: Datatypes.nat,
+     subst_trm x y (open_rec_trm n u t)
+     = open_rec_trm n (subst_fvar x y u) (subst_trm x y t)) /\
+  (forall v : val, forall n: Datatypes.nat,
+     subst_val x y (open_rec_val n u v)
+     = open_rec_val n (subst_fvar x y u) (subst_val x y v)) /\
+  (forall d : def , forall n: Datatypes.nat,
+     subst_def x y (open_rec_def n u d)
+     = open_rec_def n (subst_fvar x y u) (subst_def x y d)) /\
+  (forall ds: defs, forall n: Datatypes.nat,
+     subst_defs x y (open_rec_defs n u ds)
+     = open_rec_defs n (subst_fvar x y u) (subst_defs x y ds)).
+Proof.
+  intros. apply trm_mutind; intros; simpl; f_equal~;
+    (apply subst_open_commut_avar || apply subst_open_commut_typ_dec).
+Qed.
+
+(** - terms only *)
+Lemma subst_open_commut_trm: forall x y u t,
+    subst_trm x y (open_trm u t)
+    = open_trm (subst_fvar x y u) (subst_trm x y t).
+Proof.
+  intros. apply subst_open_commut_trm_val_def_defs.
+Qed.
+
+(** - definitions only *)
+Lemma subst_open_commut_defs: forall x y u ds,
+    subst_defs x y (open_defs u ds)
+    = open_defs (subst_fvar x y u) (subst_defs x y ds).
+Proof.
+  intros. apply subst_open_commut_trm_val_def_defs.
+Qed.
+
+(** The following lemmas state that opening a symbol with a variable [y]
+    is the same as opening the symbol with another variable [x] and
+    substituting [x] with [y]: #<br>#
+    [Z^y = (Z^x)[y/x]] *)
+
+(** Substitution after opening
+    - terms *)
+Lemma subst_intro_trm: forall x u t, x \notin (fv_trm t) ->
+  open_trm u t = subst_trm x u (open_trm x t).
+Proof.
+  introv Fr. unfold open_trm. rewrite subst_open_commut_trm.
+  destruct (@subst_fresh_trm_val_def_defs x u) as [Q _]. rewrite~ (Q t).
+  unfold subst_fvar. case_var~.
+Qed.
+
+(** - definitions *)
+Lemma subst_intro_defs: forall x u ds, x \notin (fv_defs ds) ->
+  open_defs u ds = subst_defs x u (open_defs x ds).
+Proof.
+  introv Fr. unfold open_trm. rewrite subst_open_commut_defs.
+  destruct (@subst_fresh_trm_val_def_defs x u) as [_ [_ [_ Q]]]. rewrite~ (Q ds).
+  unfold subst_fvar. case_var~.
+Qed.
+
+(** - types *)
+Lemma subst_intro_typ: forall x u T, x \notin (fv_typ T) ->
+  open_typ u T = subst_typ x u (open_typ x T).
+Proof.
+  introv Fr. unfold open_typ. rewrite subst_open_commut_typ.
+  destruct (@subst_fresh_typ_dec x u) as [Q _]. rewrite~ (Q T).
+  unfold subst_fvar. case_var~.
+Qed.
+
+Ltac subst_open_fresh :=
+  repeat match goal with
+    | [ |- context [ open_typ ?z (subst_typ ?x ?y ?T) ] ] =>
+        replace (open_typ z (subst_typ x y T)) with (open_typ (subst_fvar x y z) (subst_typ x y T))
+          by (unfold subst_fvar; rewrite~ If_r);
+        rewrite_all <- subst_open_commut_typ
+    | [ |- context [ open_defs ?z (subst_defs ?x ?y ?ds) ] ] =>
+        replace (open_defs z (subst_defs x y ds)) with (open_defs (subst_fvar x y z) (subst_defs x y ds))
+          by (unfold subst_fvar; rewrite~ If_r);
+        rewrite_all <- subst_open_commut_defs
+     | [ |- context [ open_trm ?z (subst_trm ?x ?y ?t) ] ] =>
+        replace (open_trm z (subst_trm x y t)) with (open_trm (subst_fvar x y z) (subst_trm x y t))
+          by (unfold subst_fvar; rewrite~ If_r);
+        rewrite_all <- subst_open_commut_trm
+    end.
+
+(** Substitution preserves labels of definitions: [label(d) = label(d[y/x])] *)
+Lemma subst_label_of_def: forall x y d,
+  label_of_def d = label_of_def (subst_def x y d).
+Proof.
+  intros. destruct d; reflexivity.
+Qed.
+
+(** [l \notin labels(ds)]     #<br>#
+    [――――――――――――――――――――――] #<br>#
+    [l \notin labels(ds[y/x]] *)
+Lemma subst_defs_hasnt: forall x y l ds,
+  defs_hasnt ds l ->
+  defs_hasnt (subst_defs x y ds) l.
+Proof.
+  intros x y l ds. unfold defs_hasnt. induction ds; introv Eq.
+  - reflexivity.
+  - unfold get_def. simpl. rewrite <- subst_label_of_def.
+    simpl in Eq. case_if~.
+Qed.
+
+(** [z <> x]                             #<br>#
+    [ds^z = ...{a = t}...]              #<br>#
+    [――――――――――――――――――――――――――――――――]  #<br>#
+    [(ds[y/x])^z = ...{a = t[y/x]}...]  *)
+Lemma open_subst_defs : forall x y z a ds t,
+    z <> x ->
+    defs_has (open_defs z ds) (def_trm a t) ->
+    defs_has (open_defs z (subst_defs x y ds)) (def_trm a (subst_trm x y t)).
+Proof.
+  introv. gen x y z a t. induction ds; intros.
+  - inversion H0.
+  - unfold open_defs, defs_has in *; simpls. case_if.
+    + destruct d; simpls; case_if; auto.
+      inversions H0.
+      rewrite subst_open_commut_trm. unfold subst_fvar.
+      case_if. auto.
+    + case_if; apply IHds; destruct d; auto; contradiction.
+Qed.
+
+(** [y <> x]                             #<br>#
+    [ds^x = ...{a = t}...]              #<br>#
+    [――――――――――――――――――――――――――――――――]  #<br>#
+    [(ds[y/x])^y = ...{a = t[y/x]}...]  *)
+Lemma open_subst_defs2 : forall x y a ds t,
+    y <> x ->
+    defs_has (open_defs x ds) (def_trm a t) ->
+    defs_has (open_defs y (subst_defs x y ds)) (def_trm a (subst_trm x y t)).
+Proof.
+  introv. gen x y a t. induction ds; intros.
+  - inversion H0.
+  - unfold open_defs, defs_has in *.
+    simpls; case_if; destruct d; simpls; case_if; auto.
+    subst; inversion H0.
+    rewrite subst_open_commut_trm. unfold subst_fvar. case_if; auto.
+Qed.
+
+Lemma var_typing_implies_avar_f: forall G a T,
+    G ⊢ trm_var a : T ->
+    exists x, a = avar_f x.
+Proof.
+  introv H; dependent induction H; eauto.
 Qed.
 
 Lemma fv_ctx_types_concat_eq : forall G1 G2,
@@ -904,406 +1025,4 @@ Lemma fv_ctx_types_push: forall x z T G,
 Proof.
   intros. rewrite fv_ctx_types_push_eq.
   apply notin_union. split~.
-Qed.
-
-(** [x \notin fv(G, z: T)]                   #<br>#
-    [x \notin fv(T)]                         #<br>#
-    [―――――――――――――――――――――――――――――――――――――] #<br>#
-    [x \notin fv(T)] and [x \notin fv(G)] *)
-Lemma invert_fv_ctx_types_push: forall x z T G,
-  x \notin fv_ctx_types (G & z ~ T) -> x \notin fv_typ T /\ x \notin (fv_ctx_types G).
-Proof.
-  introv H. rewrite fv_ctx_types_push_eq in H.
-  apply~ notin_union.
-Qed.
-
-(** [x \notin fv(G)]         #<br>#
-    [――――――――――――――――――]    #<br>#
-    [G[y/x] = G]    *)
-Lemma subst_fresh_ctx: forall x y G,
-  x \notin fv_ctx_types G -> subst_ctx x y G = G.
-Proof.
-  intros x y.
-  apply (env_ind (fun G => x \notin fv_ctx_types G -> subst_ctx x y G = G)).
-  + intro N. unfold subst_ctx. apply map_empty.
-  + intros G z T IH N.
-    apply invert_fv_ctx_types_push in N. destruct N as [N1 N2].
-    unfold subst_ctx in *. rewrite map_push.
-    rewrite (IH N2).
-    rewrite ((proj1 (subst_fresh_typ_dec _ _)) _ N1).
-    reflexivity.
-Qed.
-(*
-(** Definition of substitution on named variables: #<br>#
-    [z[y/x] := if z == x then y else z], where [z] is a named variable. *)
-Definition subst_fvar(x y z: var): var := If z = x then y else z.*)
-
-(** The following lemmas state that substitution commutes with opening:
-    for a symbol [Z], #<br>#
-    [(Z^a)[y/x] = (Z[y/x])^(a[y/x])]. *)
-
-(** Substitution commutes with opening
-    - variables *)
-Lemma subst_open_commut: forall x p u y n,
-    lc_path p ->
-    subst_avar x p (open_rec_avar n u y)
-    = open_rec_path_p n (subst_var_p x p u) (subst_avar x p y).
-Proof.
-  introv Hl. unfold subst_var_p, subst_avar, open_rec_avar, subst_var_p.
-  destruct y as [n' | y]; autounfold; destruct p as [z bs]; destruct z as [m | z'];
-    repeat case_if; simpl; try case_if*; eauto; inversions  Hl; inversion H0; inversion H1.
-Qed.
-
-Lemma sel_fields_open : forall n p q bs,
-  sel_fields (open_rec_path_p n p q) bs = open_rec_path_p n p (sel_fields q bs).
-Proof.
-  intros. destruct q. simpl. destruct p. destruct a. case_if; simpl; auto. rewrite* app_assoc.
-  simpl. auto.
-Qed.
-
-Lemma sel_fields_subst : forall x p y bs b,
-    subst_path x p (p_sel y bs) • b = (subst_path x p (p_sel y bs)) • b.
-Proof.
-  intros. destruct p, y; auto. simpl. unfold subst_var_p. case_if; simpl; auto.
-Qed.
-
-(** - paths *)
-Lemma subst_open_commut_path: forall p n x q u,
-    lc_path p ->
-    subst_path x p (open_rec_path n u q)
-    = open_rec_path_p n (subst_var_p x p u) (subst_path x p q).
-Proof.
-  introv Hl. destruct q as [z bs]. simpl. rewrite* subst_open_commut. rewrite* sel_fields_open.
-Qed.
-
-(** - types and declarations *)
-Lemma subst_open_commut_typ_dec: forall x p u,
-  lc_path p ->
-  (forall t : typ, forall n: nat,
-     subst_typ x p (open_rec_typ n u t)
-     = open_rec_typ_p n (subst_var_p x p u) (subst_typ x p t)) /\
-  (forall D : dec, forall n: nat,
-     subst_dec x p (open_rec_dec n u D)
-     = open_rec_dec_p n (subst_var_p x p u) (subst_dec x p D)).
-Proof.
-  intros. apply typ_mutind; intros; simpl; f_equal*. apply* subst_open_commut_path.
-Qed.
-
-Lemma subst_open_commut_p: forall x p u y n,
-    lc_path p ->
-    subst_path x p (open_rec_avar_p n u y)
-    = open_rec_path_p n (subst_path x p u) (subst_avar x p y).
-Proof.
-  introv Hl. unfold subst_path, subst_avar, subst_var_p.
-  destruct y as [n' | y]; simpl; repeat case_if; destruct u; destruct a; simpl;
-    try (rewrite* app_nil_r); repeat case_if; unfold sel_fields; destruct* p;
-      inversions Hl; inversions H0; rewrite* app_nil_l; inversion H.
-Qed.
-
-Lemma subst_open_commut_path_p: forall p n x q u,
-    lc_path q ->
-    subst_path x q (open_rec_path_p n u p)
-    = open_rec_path_p n (subst_path x q u) (subst_path x q p).
-Proof.
-  introv Hl. destruct p as [z bs]. simpl.
-  unfold subst_path. destruct u. rewrite <- sel_fields_open.
-  unfold open_rec_path_p, subst_avar.
-  destruct z; simpl; destruct a; repeat case_if*;
-    unfold subst_var_p; repeat case_if;
-      destruct q; simpl; try (rewrite app_assoc || rewrite app_nil_r);
-        inversion* Hl; subst. inversions H0. (*inversions H0. eauto. inversions H.
-        try solve [inversion Hl; inversion* H0].*)
-
-Admitted.
-
-Lemma subst_open_commut_typ_dec_p: forall x y u,
-  lc_path y ->
-  (forall t : typ, forall n: nat,
-     subst_typ x y (open_rec_typ_p n u t)
-     = open_rec_typ_p n (subst_path x y u) (subst_typ x y t)) /\
-  (forall D : dec, forall n: nat,
-     subst_dec x y (open_rec_dec_p n u D)
-     = open_rec_dec_p n (subst_path x y u) (subst_dec x y D)).
-Proof.
-  intros. apply typ_mutind; intros; simpl; f_equal*.
-  apply* subst_open_commut_path_p.
-Qed.
-
-(** - types only *)
-Lemma subst_open_commut_typ: forall x y u T,
-  lc_path y ->
-  subst_typ x y (open_typ u T) = open_typ_p (subst_var_p x y u) (subst_typ x y T).
-Proof.
-  intros. apply* subst_open_commut_typ_dec.
-Qed.
-
-Lemma subst_open_commut_typ_p: forall x y u T,
-    lc_path y ->
-    subst_typ x y (open_typ_p u T) = open_typ_p (subst_path x y u) (subst_typ x y T).
-Proof.
-  intros. apply* subst_open_commut_typ_dec_p.
-Qed.
-
-(** - terms, values, definitions, and list of definitions *)
-Lemma subst_open_commut_trm_val_def_defs: forall x y u,
-    lc_path y ->
-  (forall t : trm, forall n: nat,
-     subst_trm x y (open_rec_trm n u t)
-     = open_rec_trm_p n (subst_var_p x y u) (subst_trm x y t)) /\
-  (forall v : val, forall n: nat,
-     subst_val x y (open_rec_val n u v)
-     = open_rec_val_p n (subst_var_p x y u) (subst_val x y v)) /\
-  (forall d : def , forall n: nat,
-     subst_def x y (open_rec_def n u d)
-     = open_rec_def_p n (subst_var_p x y u) (subst_def x y d)) /\
-  (forall ds: defs, forall n: nat,
-     subst_defs x y (open_rec_defs n u ds)
-     = open_rec_defs_p n (subst_var_p x y u) (subst_defs x y ds)).
-Proof.
-  intros. apply trm_mutind; intros; simpl; f_equal*;
-  apply* subst_open_commut_path || apply* subst_open_commut_typ_dec.
-Qed.
-
-Lemma subst_open_commut_trm_val_def_defs_p: forall x y u,
-    lc_path y ->
-  (forall t : trm, forall n: nat,
-     subst_trm x y (open_rec_trm_p n u t)
-     = open_rec_trm_p n (subst_path x y u) (subst_trm x y t)) /\
-  (forall v : val, forall n: nat,
-     subst_val x y (open_rec_val_p n u v)
-     = open_rec_val_p n (subst_path x y u) (subst_val x y v)) /\
-  (forall d : def , forall n: nat,
-     subst_def x y (open_rec_def_p n u d)
-     = open_rec_def_p n (subst_path x y u) (subst_def x y d)) /\
-  (forall ds: defs, forall n: nat,
-     subst_defs x y (open_rec_defs_p n u ds)
-     = open_rec_defs_p n (subst_path x y u) (subst_defs x y ds)).
-Proof.
-  intros. apply trm_mutind; intros; simpl; f_equal*;
-  apply* subst_open_commut_typ_dec_p || apply* subst_open_commut_path_p.
-Qed.
-
-(** - terms only *)
-Lemma subst_open_commut_trm: forall x y u t,
-    lc_path y ->
-    subst_trm x y (open_trm u t)
-    = open_trm_p (subst_var_p x y u) (subst_trm x y t).
-Proof.
-  intros. apply* subst_open_commut_trm_val_def_defs.
-Qed.
-
-Lemma subst_open_commut_trm_p: forall x y u t,
-    lc_path y ->
-    subst_trm x y (open_trm_p u t)
-    = open_trm_p (subst_path x y u) (subst_trm x y t).
-Proof.
-  intros. apply* subst_open_commut_trm_val_def_defs_p.
-Qed.
-
-(** - definitions only *)
-Lemma subst_open_commut_defs: forall x y u ds,
-    lc_path y ->
-    subst_defs x y (open_defs u ds)
-    = open_defs_p (subst_var_p x y u) (subst_defs x y ds).
-Proof.
-  intros. apply* subst_open_commut_trm_val_def_defs.
-Qed.
-
-Lemma subst_open_commut_defs_p: forall x y u ds,
-    lc_path y ->
-    subst_defs x y (open_defs_p u ds)
-    = open_defs_p (subst_path x y u) (subst_defs x y ds).
-Proof.
-  intros. apply* subst_open_commut_trm_val_def_defs_p.
-Qed.
-
-(** The following lemmas state that opening a symbol with a variable [y]
-    is the same as opening the symbol with another variable [x] and
-    substituting [x] with [y]: #<br>#
-    [Z^y = (Z^x)[y/x]] *)
-
-(** Substitution after opening
-    - terms *)
-Lemma subst_intro_trm: forall x u t, x \notin (fv_trm t) -> lc_path u ->
-  open_trm_p u t = subst_trm x u (open_trm x t).
-Proof.
-  introv Fr Hl. unfold open_trm. rewrite* subst_open_commut_trm.
-  destruct (@subst_fresh_trm_val_def_defs x u) as [Q _]. rewrite~ (Q t).
-  unfold subst_var_p. case_var~.
-Qed.
-
-(** - definitions *)
-Lemma subst_intro_defs: forall x u ds, x \notin (fv_defs ds) -> lc_path u ->
-  open_defs_p u ds = subst_defs x u (open_defs x ds).
-Proof.
-  introv Fr Hl. unfold open_trm. rewrite* subst_open_commut_defs.
-  destruct (@subst_fresh_trm_val_def_defs x u) as [_ [_ [_ Q]]]. rewrite~ (Q ds).
-  unfold subst_var_p. case_var~.
-Qed.
-
-(** - types *)
-Lemma subst_intro_typ: forall x u T, x \notin (fv_typ T) -> lc_path u ->
-  open_typ_p u T = subst_typ x u (open_typ x T).
-Proof.
-  introv Fr Hl. unfold open_typ. rewrite* subst_open_commut_typ.
-  destruct (@subst_fresh_typ_dec x u) as [Q _]. rewrite* (Q T).
-  unfold subst_var_p. case_var*.
-Qed.
-
-Ltac subst_open_fresh :=
-  match goal with
-  | [ |- context [ open_typ ?z (subst_typ ?x ?p ?T) ] ] =>
-    replace (open_typ z (subst_typ x p T)) with (open_typ_p (subst_path x p (pvar z)) (subst_typ x p T)) by
-        (unfold subst_path; simpl; unfold subst_var_p; rewrite If_r, open_var_typ_eq; auto)
-    | [ |- context [ open_defs ?z (subst_defs ?x ?p ?ds) ] ] =>
-        replace (open_defs z (subst_defs x p ds)) with (open_defs_p (subst_path x p (pvar z)) (subst_defs x p ds))
-          by (unfold subst_path; simpl; unfold subst_var_p; rewrite If_r, open_var_defs_eq; auto)
-     | [ |- context [ open_trm ?z (subst_trm ?x ?p ?t) ] ] =>
-        replace (open_trm z (subst_trm x p t)) with (open_trm_p (subst_path x p (pvar z)) (subst_trm x p t))
-          by (unfold subst_path; simpl; unfold subst_var_p; rewrite If_r, open_var_trm_eq; auto)
-    end.
-
-(** Substitution preserves labels of definitions: [label(d) = label(d[y/x])] *)
-Lemma subst_label_of_def: forall x y d,
-  label_of_def d = label_of_def (subst_def x y d).
-Proof.
-  intros. destruct* d.
-Qed.
-
-(** [l \notin labels(ds)]     #<br>#
-    [――――――――――――――――――――――] #<br>#
-    [l \notin labels(ds[y/x]] *)
-Lemma subst_defs_hasnt: forall x y l ds,
-  defs_hasnt ds l ->
-  defs_hasnt (subst_defs x y ds) l.
-Proof.
-  intros x y l ds. unfold defs_hasnt. induction ds; introv Eq; auto.
-  unfold get_def. simpl. rewrite <- subst_label_of_def.
-  simpl in Eq. case_if~.
-Qed.
-
-(** Definition of substitution on named variables: #<br>#
-    [z[y/x] := if z == x then y else z], where [z] is a named variable. *)
-Definition subst_fvar(x y z: var): var := If z = x then y else z.
-
-
-(** [z <> x]                             #<br>#
-    [ds^z = ...{a = t}...]              #<br>#
-    [――――――――――――――――――――――――――――――――]  #<br>#
-    [(ds[y/x])^z = ...{a = t[y/x]}...]  *)
-Lemma open_subst_defs : forall x y z a ds t,
-    z <> x ->
-    defs_has (open_defs z ds) (def_trm a t) ->
-    defs_has (open_defs z (subst_defs x y ds)) (def_trm a (subst_trm x y t)).
-Proof.
-  introv. gen x y z a t. induction ds; intros.
-  - inversion H0.
-  - unfold open_defs, defs_has in *; simpls. case_if.
-    + destruct d; simpls; case_if; auto.
-      inversions H0.
-      rewrite subst_open_commut_trm. unfold subst_fvar.
-      Admitted. (*case_if. auto.
-    + case_if; apply IHds; destruct d; auto; contradiction.
-Qed.*)
-
-(** [y <> x]                             #<br>#
-    [ds^x = ...{a = t}...]              #<br>#
-    [――――――――――――――――――――――――――――――――]  #<br>#
-    [(ds[y/x])^y = ...{a = t[y/x]}...]  *)
-(*Lemma open_subst_defs2 : forall x y a ds t,
-    y <> x ->
-    defs_has (open_defs x ds) (def_trm a t) ->
-    defs_has (open_defs y (subst_defs x y ds)) (def_trm a (subst_trm x y t)).
-Proof.
-  introv. gen x y a t. induction ds; intros.
-  - inversion H0.
-  - unfold open_defs, defs_has in *.
-    simpls; case_if; destruct d; simpls; case_if; auto.
-    subst; inversion H0.
-    rewrite subst_open_commut_trm. unfold subst_fvar. case_if; auto.
-Qed.
-*)
-
-(** - variables *)
-
-Lemma open_fresh_path_injective : forall p q k z,
-    z \notin fv_path p ->
-    z \notin fv_path q ->
-    open_rec_path k z p = open_rec_path k z q ->
-    p = q.
-Proof.
-  intros. destruct p, q. inversions* H1. simpl in *; f_equal.
-  Admitted.
-
- Ltac invert_open :=
-    match goal with
-    | [ H: _ = open_rec_typ _ _ ?T' |- _ ] =>
-       destruct T'; inversions* H
-    | [ H: _ = open_rec_dec _ _ ?D' |- _ ] =>
-       destruct D'; inversions* H
-    end.
-
-(** - types and declarations *)
-Lemma open_fresh_typ_dec_injective:
-  (forall T T' k x,
-    x \notin fv_typ T ->
-    x \notin fv_typ T' ->
-    open_rec_typ k x T = open_rec_typ k x T' ->
-    T = T') /\
-  (forall D D' k x,
-    x \notin fv_dec D ->
-    x \notin fv_dec D' ->
-    open_rec_dec k x D = open_rec_dec k x D' ->
-    D = D').
-Proof.
-  apply typ_mutind; intros; invert_open; simpl in *;
-    f_equal; eauto using open_fresh_avar_injective, open_fresh_path_injective.
-Qed.
-
-Lemma open_fresh_trm_val_def_defs_injective:
-  (forall t t' k x,
-      x \notin fv_trm t ->
-      x \notin fv_trm t' ->
-      open_rec_trm k x t = open_rec_trm k x t' ->
-      t = t') /\
-  (forall v v' k x,
-      x \notin fv_val v ->
-      x \notin fv_val v' ->
-      open_rec_val k x v = open_rec_val k x v' ->
-      v = v') /\
-  (forall d d' k x,
-      x \notin fv_def d ->
-      x \notin fv_def d' ->
-      open_rec_def k x d = open_rec_def k x d' ->
-      d = d') /\
-  (forall ds ds' k x,
-      x \notin fv_defs ds ->
-      x \notin fv_defs ds' ->
-      open_rec_defs k x ds = open_rec_defs k x ds' ->
-      ds = ds').
-Proof.
-
-  Ltac injective_solver :=
-    match goal with
-    | [ H: _ = open_rec_trm _ _ ?t |- _ ] =>
-      destruct t; inversions H;
-      try (f_equal; simpl in *);
-           try (apply* open_fresh_avar_injective || apply* open_fresh_path_injective);
-           match goal with
-           | [ Ho: open_rec_avar _ _ _ = open_rec_avar _ _ _ |- _ ] =>
-             apply open_fresh_avar_injective in Ho; subst*
-           | [ Heq: forall _ _ _, _ -> _ -> _ -> ?u = _ |- ?u = _ ] =>
-             apply* Heq
-           end
-    | [ H: _ = open_rec_val _ _ ?v |- _ ] =>
-      destruct v; inversions H; f_equal; simpl in *;
-      try apply* open_fresh_typ_dec_injective; eauto
-    | [ H: _ = open_rec_def _ _ ?d |- _ ] =>
-      destruct d; inversions H; f_equal;
-      try apply* open_fresh_typ_dec_injective; eauto
-    | [ H: _ = open_rec_defs _ _ ?ds |- _ ] =>
-      destruct ds; inversions H; f_equal; simpl in *; eauto
-    end.
-
-  apply trm_mutind; intros; try solve [injective_solver].
 Qed.
