src/paths-new/Definitions.v
@@ -121,6 +121,8 @@ Definition sel_fields (p : path) (bs : list trm_label) :=
   end.
 Notation "p '•' a" := (sel_fields p (a :: nil)) (at level 5).
 
+Hint Unfold pavar pvar tvar.
+
 (** Helper functions to retrieve labels of declarations and definitions *)
 
 Definition label_of_def(d: def): label := match d with
@@ -764,6 +766,49 @@ Inductive wf_sto: ctx -> ec -> Prop :=
     G ⊢ trm_val v : T ->
     G & x ~ T ~~ s & x ~ v
 where "G '~~' s" := (wf_sto G s).
+
+Reserved Notation "e '∋' t" (at level 60).
+
+Inductive lookup : ec -> path * val -> Prop :=
+
+(** [e(x) = v  ]    #<br>#
+    [――――――――――]    #<br>#
+    [e ∋ (x, v)]    *)
+| lookup_ec : forall e x v,
+    binds x v e ->
+    e ∋ (pvar x, v)
+
+(** [e ∋ (p, ν(T)...{ b = v }...)]    #<br>#
+    [――――――――――――――――――――――――――――]    #<br>#
+    [e ∋ (p.b, v)                ]    *)
+| lookup_val : forall e p b T ds v,
+    e ∋ (p, val_new T ds) ->
+    get_def (label_trm b) ds = Some (def_trm b (trm_val v)) ->
+    e ∋ (p•b, v)
+
+(** [e ∋ (p, ν(T)...{ b = x.bs }...)] #<br>#
+    [e ∋ (x.bs, v)                  ] #<br>#
+    [―――――――――――――――――――――――――――――――] #<br>#
+    [e ∋ (p.b, v)                   ] *)
+| lookup_x : forall e p T ds b x bs v,
+    e ∋ (p, val_new T ds) ->
+    get_def (label_trm b) ds = Some (def_trm b (trm_path (p_sel (avar_f x) bs))) ->
+    e ∋ (p_sel (avar_f x) bs, v) ->
+    e ∋ (p•b, v)
+
+(** [e ∋ (p, ν(T)...{ b = n.bs }...)] #<br>#
+    [e ∋ ((p drop n).bs, v)         ] #<br>#
+    [―――――――――――――――――――――――――――――――] #<br>#
+    [e ∋ (p.b, v)                   ] *)
+| lookup_n : forall e p T ds b x bs v cs n,
+    e ∋ (p, val_new T ds) ->
+    get_def (label_trm b) ds = Some (def_trm b (trm_path (p_sel (avar_b n) bs))) ->
+    p = p_sel x cs ->
+    (* `skipn n cs` removes the n last fields of the path, yielding the path to bs *)
+    e ∋ (p_sel x (bs ++ skipn n cs), v) ->
+    e ∋ (p•b, v)
+
+where "e '∋' t" := (lookup e t).
 
 (** * Typing Relations for the Safety Proof *)
 (** The following typing relations are not part of the DOT calculus, but are used
