src/simple-proof/proof-stacks/GeneralToTight.v
@@ -1,7 +1,7 @@
-(** printing |-#    %\vdash_{\#}%    #&vdash;<sub>&#35;</sub>#     *)
-(** printing |-##   %\vdash_{\#\#}%  #&vdash;<sub>&#35&#35</sub>#  *)
-(** printing |-##v  %\vdash_{\#\#v}% #&vdash;<sub>&#35&#35v</sub># *)
-(** printing |-!    %\vdash_!%       #&vdash;<sub>!</sub>#         *)
+(** printing ⊢#    %\vdash_{\#}%    #&vdash;<sub>&#35;</sub>#     *)
+(** printing ⊢##   %\vdash_{\#\#}%  #&vdash;<sub>&#35&#35</sub>#  *)
+(** printing ⊢##v  %\vdash_{\#\#v}% #&vdash;<sub>&#35&#35v</sub># *)
+(** printing ⊢!    %\vdash_!%       #&vdash;<sub>!</sub>#         *)
 (** remove printing ~ *)
 
 Set Implicit Arguments.
@@ -9,23 +9,25 @@ Set Implicit Arguments.
 Require Import LibLN.
 Require Import Coq.Program.Equality.
 Require Import Definitions.
+Require Import RecordAndInertTypes.
 Require Import PreciseTypes.
-Require Import InvertibleTyping.
+Require Import TightTypes.
+Require Import InvertibleTypes.
 
 (** * Sel-<: Premise
     This lemma corresponds to Lemma 3.5 in the paper.
 
     [inert G]                    #<br>#
-    [G |-## x: {A: S..U}]        #<br>#
+    [G ⊢## x: {A: S..U}]        #<br>#
     [――――――――――――――――――――――――――――]   #<br>#
-    [exists T. G |-## x: {A: T..T}]   #<br>#
-    [G |-# T <: U]               #<br>#
-    [G |-# S <: T]                    *)
-Lemma sel_premise: forall G p A S U,
+    [exists T. G ⊢## x: {A: T..T}]   #<br>#
+    [G ⊢# T <: U]               #<br>#
+    [G ⊢# S <: T]                    *)
+Lemma sel_premise: forall G x A S U,
   inert G ->
-  G ⊢## p : typ_rcd (dec_typ A S U) ->
+  G ⊢## x : typ_rcd (dec_typ A S U) ->
   exists T,
-    G ⊢! trm_path p : typ_rcd (dec_typ A T T) /\
+    G ⊢! trm_var (avar_f x) : typ_rcd (dec_typ A T T) /\
     G ⊢# T <: U /\
     G ⊢# S <: T.
 Proof.
@@ -33,7 +35,7 @@ Proof.
   dependent induction Hinv.
   - lets Hp: (precise_dec_typ_inv HG H). subst.
     exists U. split*.
-  - specialize (IHHinv _ _ _ HG eq_refl).
+  - specialize (IHHinv A T U0 HG eq_refl).
     destruct IHHinv as [V [Hx [Hs1 Hs2]]].
     exists V. split*.
 Qed.
@@ -46,11 +48,11 @@ Qed.
     [――――――――――――――――――――――]   #<br>#
     [G ⊢# x.A <: U]       #<br>#
     [G ⊢# S <: x.A]            *)
-Lemma sel_replacement: forall G p A S U,
+Lemma sel_replacement: forall G x A S U,
     inert G ->
-    G ⊢# trm_path p : typ_rcd (dec_typ A S U) ->
-    (G ⊢# typ_path p A <: U /\
-     G ⊢# S <: typ_path p A).
+    G ⊢# trm_var (avar_f x) : typ_rcd (dec_typ A S U) ->
+    (G ⊢# typ_sel (avar_f x) A <: U /\
+     G ⊢# S <: typ_sel (avar_f x) A).
 Proof.
   introv HG Hty.
   pose proof (tight_to_invertible HG Hty) as Hinv.
