src/simple-proof/proof-stacks/InvertibleTypes.v
@@ -1,0 +1,299 @@
+(** printing ⊢#    %\vdash_{\#}%    #&vdash;<sub>&#35;</sub>#     *)
+(** printing ⊢##   %\vdash_{\#\#}%  #&vdash;<sub>&#35&#35</sub>#  *)
+(** printing ⊢##v  %\vdash_{\#\#v}% #&vdash;<sub>&#35&#35v</sub># *)
+(** printing ⊢!    %\vdash_!%       #&vdash;<sub>!</sub>#         *)
+(** remove printing ~ *)
+
+(** This module contains lemmas related to invertible typing
+    ([ty_var_inv], [⊢##] and [ty_val_inv], [⊢##v]). *)
+
+Set Implicit Arguments.
+
+Require Import LibLN.
+Require Import Coq.Program.Equality.
+Require Import Definitions.
+Require Import RecordAndInertTypes.
+Require Import SubEnvironments.
+Require Import Narrowing.
+Require Import PreciseTypes.
+Require Import TightTypes.
+
+(** The invertible-typing relation describes the possible types that a variable or value
+can be typed with in an inert context. For example, if [G] is inert, [G ⊢! x: {a: T}],
+and [G ⊢ T <: T'], then [G ⊢## x: {a: T'}].
+
+The purpose of invertible typing is to be easily invertible into a precise typing relation.
+To achieve that, invertible typing avoids typing cycles that could result from, for example,
+repeated applications of recursion introduction and elimination.
+For this case, invertible typing defines only recursion introduction (whereas precise typing
+defines only recursion elimination). *)
+
+(** * Invertible typing of variables [G ⊢## x: T] *)
+
+Reserved Notation "G '⊢##' x ':' T" (at level 40, x at level 59).
+
+Inductive ty_var_inv : ctx -> var -> typ -> Prop :=
+
+(** [G ⊢! x: T]  #<br>#
+    [―――――――――――] #<br>#
+    [G ⊢## x: T]     *)
+| ty_precise_inv : forall G x T,
+  G ⊢! trm_var (avar_f x) : T ->
+  G ⊢## x : T
+
+(** [G ⊢## x: {a: T}] #<br>#
+    [G ⊢# T <: U]     #<br>#
+    [――――――――――――――――] #<br>#
+    [G ⊢## x: {a: U}]     *)
+| ty_dec_trm_inv : forall G x a T U,
+  G ⊢## x : typ_rcd (dec_trm a T) ->
+  G ⊢# T <: U ->
+  G ⊢## x : typ_rcd (dec_trm a U)
+
+(** [G ⊢## x: {A: T..U}]   #<br>#
+    [G ⊢# T' <: T]         #<br>#
+    [G ⊢# U <: U']         #<br>#
+    [―――――――――――――――――――――] #<br>#
+    [G ⊢## x: {A: T'..U'}]     *)
+| ty_dec_typ_inv : forall G x A T T' U' U,
+  G ⊢## x : typ_rcd (dec_typ A T U) ->
+  G ⊢# T' <: T ->
+  G ⊢# U <: U' ->
+  G ⊢## x : typ_rcd (dec_typ A T' U')
+
+(** [G ⊢## x: T^x]   #<br>#
+    [―――――――――――――――] #<br>#
+    [G ⊢## x: mu(T)] *)
+| ty_bnd_inv : forall G x T,
+  G ⊢## x : open_typ x T ->
+  G ⊢## x : typ_bnd T
+
+(** [G ⊢## x: forall(S)T]          #<br>#
+    [G ⊢# S' <: S]            #<br>#
+    [G, y: S' ⊢ T^y <: T'^y]   #<br>#
+    [y fresh]                  #<br>#
+    [――――――――――――――――――――――]   #<br>#
+    [G ⊢## x: forall(S')T']            *)
+| ty_all_inv : forall L G x S T S' T',
+  G ⊢## x : typ_all S T ->
+  G ⊢# S' <: S ->
+  (forall y, y \notin L ->
+   G & y ~ S' ⊢ open_typ y T <: open_typ y T') ->
+  G ⊢## x : typ_all S' T'
+
+(** [G ⊢## x : T]     #<br>#
+    [G ⊢## x : U]     #<br>#
+    [――――――――――――――――] #<br>#
+    [G ⊢## x : T /\ U]      *)
+| ty_and_inv : forall G x S1 S2,
+  G ⊢## x : S1 ->
+  G ⊢## x : S2 ->
+  G ⊢## x : typ_and S1 S2
+
+(** [G ⊢## x: S]        #<br>#
+    [G ⊢! y: {A: S..S}] #<br>#
+    [――――――――――――――――――] #<br>#
+    [G ⊢## x: y.A           *)
+| ty_sel_inv : forall G x y A S,
+  G ⊢## x : S ->
+  G ⊢! trm_var y : typ_rcd (dec_typ A S S) ->
+  G ⊢## x : typ_sel y A
+
+(** [G ⊢## x: T]   #<br>#
+    [―――――――――――――] #<br>#
+    [G ⊢## x: top]     *)
+| ty_top_inv : forall G x T,
+  G ⊢## x : T ->
+  G ⊢## x : typ_top
+where "G '⊢##' x ':' T" := (ty_var_inv G x T).
+
+(** *** Invertible typing of values [G ⊢##v v: T] *)
+
+Reserved Notation "G '⊢##v' v ':' T" (at level 40, v at level 59).
+
+Inductive ty_val_inv : ctx -> val -> typ -> Prop :=
+
+(** [G ⊢! v: T]    #<br>#
+    [―――――――――――――] #<br>#
+    [G ⊢##v v: T] *)
+| ty_precise_inv_v : forall G v T,
+  G ⊢! trm_val v : T ->
+  G ⊢##v v : T
+
+(** [G ⊢##v v: forall(S)T]          #<br>#
+    [G ⊢# S' <: S]             #<br>#
+    [G, y: S' ⊢ T^y <: T'^y]    #<br>#
+    [y fresh]                   #<br>#
+    [――――――――――――――――――――――]    #<br>#
+    [G ⊢##v v: forall(S')T']            *)
+| ty_all_inv_v : forall L G v S T S' T',
+  G ⊢##v v : typ_all S T ->
+  G ⊢# S' <: S ->
+  (forall y, y \notin L ->
+   G & y ~ S' ⊢ open_typ y T <: open_typ y T') ->
+  G ⊢##v v : typ_all S' T'
+
+(** [G ⊢##v v: S]       #<br>#
+    [G ⊢! y: {A: S..S}] #<br>#
+    [――――――――――――――――――] #<br>#
+    [G ⊢##v v: y.A]         *)
+| ty_sel_inv_v : forall G v y A S,
+  G ⊢##v v : S ->
+  G ⊢! trm_var y : typ_rcd (dec_typ A S S) ->
+  G ⊢##v v : typ_sel y A
+
+(** [G ⊢##v v : T]        #<br>#
+    [G ⊢##v v : U]        #<br>#
+    [―――――――――――――]        #<br>#
+    [G ⊢##v v : T /\ U]        *)
+| ty_and_inv_v : forall G v T U,
+  G ⊢##v v : T ->
+  G ⊢##v v : U ->
+  G ⊢##v v : typ_and T U
+
+(** [G ⊢##v v: T]   #<br>#
+    [――――――――――――――] #<br>#
+    [G ⊢##v v: top]     *)
+| ty_top_inv_v : forall G v T,
+  G ⊢##v v : T ->
+  G ⊢##v v : typ_top
+where "G '⊢##v' v ':' T" := (ty_val_inv G v T).
+
+Hint Constructors ty_var_inv ty_val_inv.
+
+(** ** Invertible to Precise Typing [|-## to |-!] *)
+
+(** Invertible-to-precise typing for field declarations: #<br>#
+    [G ⊢## x: {a: T}]            #<br>#
+    [――――――――――――――――――――――]      #<br>#
+    [exists T', G ⊢! x: {a: T'}]      #<br>#
+    [G ⊢# T' <: T]. *)
+Lemma invertible_to_precise_trm_dec: forall G x a T,
+  G ⊢## x : typ_rcd (dec_trm a T) ->
+  exists T',
+    G ⊢! trm_var (avar_f x) : typ_rcd (dec_trm a T') /\
+    G ⊢# T' <: T.
+Proof.
+  introv Hinv.
+  dependent induction Hinv.
+  - exists T. auto.
+  - specialize (IHHinv _ _ eq_refl). destruct IHHinv as [V [Hx Hs]].
+    exists V. split; auto.
+    eapply subtyp_trans_t; eassumption.
+Qed.
+
+(** Invertible-to-precise typing for function types: #<br>#
+    [ok G]                        #<br>#
+    [G ⊢## x: forall(S)T]             #<br>#
+    [――――――――――――――――――――――――――]  #<br>#
+    [exists S', T'. G ⊢! x: forall(S')T']  #<br>#
+    [G ⊢# S <: S']               #<br>#
+    [G ⊢# T'^y <: T^y], where [y] is fresh. *)
+Lemma invertible_to_precise_typ_all: forall G x S T,
+  ok G ->
+  G ⊢## x : typ_all S T ->
+  exists S' T' L,
+    G ⊢! trm_var (avar_f x) : typ_all S' T' /\
+    G ⊢# S <: S' /\
+    (forall y,
+        y \notin L ->
+            G & y ~ S ⊢ open_typ y T' <: open_typ y T).
+Proof.
+  introv HG Hinv.
+  dependent induction Hinv.
+  - exists S T (dom G); auto.
+  - specialize (IHHinv _ _ HG eq_refl).
+    destruct IHHinv as [S' [T' [L' [Hpt [HSsub HTsub]]]]].
+    exists S' T' (dom G \u L \u L').
+    split; auto.
+    assert (Hsub2 : G ⊢# typ_all S0 T0 <: typ_all S T).
+    { apply subtyp_all_t with (L:=L); assumption. }
+    split.
+    + eapply subtyp_trans_t; eauto.
+    + intros y Fr.
+      assert (Hok: ok (G & y ~ S)) by auto using ok_push.
+      apply tight_to_general in H; auto.
+      assert (Hnarrow: G & y ~ S ⊢ open_typ y T' <: open_typ y T0).
+      { eapply narrow_subtyping; auto using subenv_last. }
+      eauto.
+Qed.
+
+(** ** Invertible Subtyping Closure *)
+
+(** Invertible typing is closed under tight subtyping. *)
+Lemma invertible_typing_closure_tight: forall G x T U,
+  inert G ->
+  G ⊢## x : T ->
+  G ⊢# T <: U ->
+  G ⊢## x : U.
+Proof.
+  intros G x T U Hgd HT Hsub.
+  dependent induction Hsub; eauto.
+  - inversion HT.
+    destruct (precise_bot_false Hgd H).
+  - inversion HT; auto. apply ty_and1_p in H. auto.
+  - inversion HT; auto. apply ty_and2_p in H. auto.
+  - inversions HT.
+    + false* precise_psel_false.
+    + pose proof (inert_unique_tight_bounds Hgd H H5) as Hu. subst. assumption.
+Qed.
+
+(** ** Tight-to-Invertible Lemma for Variables [|-# to |-##]
+
+       This lemma corresponds to Theorem 3.6 in the paper.
+
+       [inert G]            #<br>#
+       [G ⊢# x: U]         #<br>#
+       [―――――――――――――――]    #<br>#
+       [G ⊢## x: U] *)
+Lemma tight_to_invertible :
+  forall G U x,
+    inert G ->
+    G ⊢# trm_var (avar_f x) : U ->
+    G ⊢## x : U.
+Proof.
+  intros G U x Hgd Hty.
+  dependent induction Hty.
+  - auto.
+  - specialize (IHHty _ Hgd eq_refl).
+    eapply ty_bnd_inv.
+    apply IHHty.
+  - specialize (IHHty _ Hgd eq_refl).
+    inversion IHHty; subst; auto.
+  - apply ty_and_inv; auto.
+  - eapply invertible_typing_closure_tight; auto.
+Qed.
+
+(** * Invertible Value Typing *)
+
+(** ** Invertible Subtyping Closure *)
+
+(** Invertible value typing is closed under tight subtyping. *)
+Lemma invertible_typing_closure_tight_v: forall G v T U,
+  inert G ->
+  G ⊢##v v : T ->
+  G ⊢# T <: U ->
+  G ⊢##v v : U.
+Proof.
+  introv Hgd HT Hsub.
+  dependent induction Hsub; eauto; inversions HT; auto; try solve [inversion* H].
+  - inversions H0.
+  - lets Hb: (inert_unique_tight_bounds Hgd H H5). subst*.
+Qed.
+
+(** ** Tight-to-Invertible Lemma for Values [|-# to |-##]
+
+       [inert G]            #<br>#
+       [G ⊢# v: T]         #<br>#
+       [――――――――――――――――]   #<br>#
+       [G ⊢##v v: T] *)
+Lemma tight_to_invertible_v : forall G v T,
+    inert G ->
+    G ⊢# trm_val v : T ->
+    G ⊢##v v : T.
+Proof.
+  introv Hgd Hty.
+  dependent induction Hty; eauto.
+  specialize (IHHty v Hgd eq_refl).
+  apply* invertible_typing_closure_tight_v.
+Qed.
