src/simple-proof/proof-stacks/Narrowing.v
@@ -1,0 +1,120 @@
+(** printing ⊢#    %\vdash_{\#}%    #&vdash;<sub>&#35;</sub>#     *)
+(** printing ⊢##   %\vdash_{\#\#}%  #&vdash;<sub>&#35&#35</sub>#  *)
+(** printing ⊢##v  %\vdash_{\#\#v}% #&vdash;<sub>&#35&#35v</sub># *)
+(** printing ⊢!    %\vdash_!%       #&vdash;<sub>!</sub>#         *)
+(** remove printing ~ *)
+
+Set Implicit Arguments.
+
+Require Import LibLN.
+Require Import Definitions.
+Require Import SubEnvironments.
+Require Import Weakening.
+Require Import Coq.Program.Equality.
+
+
+(** * Narrowing Lemma *)
+(** The narrowing lemma states that typing is preserved under subenvironments.
+    The lemma corresponds to Lemma 3.11 in the paper.
+    The proof is by mutual induction on term typing, definition typing,
+    and subtyping. *)
+
+(** [G ⊢ t: T]                 #<br>#
+    [G' subG G]                #<br>#
+    [ok G']                    #<br>#
+    [―――――――――――――――――]        #<br>#
+    [G' ⊢ t: T]
+
+    and
+
+    [G ⊢ d: D]                 #<br>#
+    [G' subG G]                #<br>#
+    [ok G']                    #<br>#
+    [―――――――――――――――――]        #<br>#
+    [G' ⊢ d: D]
+
+    and
+
+    [G ⊢ ds :: T]              #<br>#
+    [G' subG G]                #<br>#
+    [ok G']                    #<br>#
+    [―――――――――――――――――]        #<br>#
+    [G' ⊢ ds :: T]
+
+    and
+
+    [G ⊢ S <: U]               #<br>#
+    [G' subG G]                #<br>#
+    [ok G']                    #<br>#
+    [―――――――――――――――――]        #<br>#
+    [G' ⊢ S <: U]              #<br>#
+
+Note: for simplicity, the definition typing judgements and [ok] conditions
+      are omitted from the paper formulation. *)
+Lemma narrow_rules:
+  (forall G t T, G ⊢ t : T -> forall G',
+    G' ⪯ G ->
+    G' ⊢ t : T)
+/\ (forall G d D, G /- d : D -> forall G',
+    G' ⪯ G ->
+    G' /- d : D)
+/\ (forall G ds T, G /- ds :: T -> forall G',
+    G' ⪯ G ->
+    G' /- ds :: T)
+/\ (forall G S U, G ⊢ S <: U -> forall G',
+    G' ⪯ G ->
+    G' ⊢ S <: U).
+Proof.
+  apply rules_mutind; intros; eauto 4;
+    try solve [
+          match goal with
+          | [ H : _ ⪯ _ |- _ ] => destruct (subenv_implies_ok H)
+          end;
+          fresh_constructor].
+
+  Case "ty_var".
+  induction H; auto;
+  match goal with
+  | [ H : binds _ _ (_ & _) |- _ ] =>
+    apply binds_push_inv in H; destruct_all; subst
+  end;
+  [ eapply ty_sub; [eauto 2 | apply weaken_subtyp; trivial]
+  | apply weaken_ty_trm; auto].
+Qed.
+
+
+(** The narrowing lemma, formulated only for term typing. *)
+Lemma narrow_typing: forall G G' t T,
+  G ⊢ t : T ->
+  G' ⪯ G ->
+  G' ⊢ t : T.
+Proof.
+  intros. apply* narrow_rules.
+Qed.
+
+(** The narrowing lemma, formulated only for subtyping. *)
+Lemma narrow_subtyping: forall G G' S U,
+  G ⊢ S <: U ->
+  G' ⪯ G ->
+  G' ⊢ S <: U.
+Proof.
+  intros. apply* narrow_rules.
+Qed.
+
+(** The subenvironment relation [⪯] is transitive.*)
+Lemma subenv_trans : forall G1 G2 G3,
+    G1 ⪯ G2 ->
+    G2 ⪯ G3 ->
+    G1 ⪯ G3.
+Proof.
+  introv H. gen G3. induction H; intros; auto.
+  dependent induction H3.
+  - apply empty_push_inv in x. contradiction.
+  - rename x into He. apply eq_push_inv in He. destruct_all.
+    subst.
+    apply IHsubenv in H3.
+    constructor; auto.
+    apply narrow_subtyping with (G':=G) in H6; auto.
+    eapply subtyp_trans; eauto.
+Qed.
+Hint Resolve subenv_trans.
