src/simple-proof/proof-stacks/PreciseTypes.v
@@ -1,0 +1,482 @@
+(** printing ⊢#    %\vdash_{\#}%    #&vdash;<sub>&#35;</sub>#     *)
+(** printing ⊢##   %\vdash_{\#\#}%  #&vdash;<sub>&#35&#35</sub>#  *)
+(** printing ⊢##v  %\vdash_{\#\#v}% #&vdash;<sub>&#35&#35v</sub># *)
+(** printing ⊢!    %\vdash_!%       #&vdash;<sub>!</sub>#         *)
+(** remove printing ~ *)
+
+(** This module reasons about the precise types of variables in inert contexts. *)
+
+Set Implicit Arguments.
+
+Require Import LibLN.
+Require Import Coq.Program.Equality.
+Require Import Definitions.
+Require Import RecordAndInertTypes.
+
+(** * Precise typing [G ⊢! t: T] *)
+(** Precise typing is used to reason about the types of variables and values.
+    Precise typing does not "modify" a variable's or value's type through subtyping.
+    - For values, precise typing allows to only retrieve the "immediate" type of the value.
+      It types objects with recursive types, and functions with dependent-function types. #<br>#
+      For example, if a value is the object [nu(x: {a: T}){a = x.a}], the only way to type
+      the object through precise typing is [G ⊢! nu(x: {a: T}){a = x.a}: mu(x: {a: T})].
+    - For variables, we start out with a type [T=G(x)] (the type to which the variable is
+      bound in [G]). Then we use precise typing to additionally deconstruct [T]
+      by using recursion elimination and intersection elimination. #<br>#
+      For example, if [G(x)=mu(x: {a: T} /\ {B: S..U})], then we can derive the following
+      precise types for [x]:               #<br>#
+      [G ⊢! x: mu(x: {a: T} /\ {B: S..U})] #<br>#
+      [G ⊢! x: {a: T} /\ {B: S..U}]        #<br>#
+      [G ⊢! x: {a: T}]                    #<br>#
+      [G ⊢! x: {B: S..U}].                *)
+
+Reserved Notation "G '⊢!' t ':' T" (at level 40, t at level 59).
+
+Inductive ty_trm_p : ctx -> trm -> typ -> Prop :=
+
+(** [G(x) = T]      #<br>#
+    [―――――――――――――] #<br>#
+    [G ⊢! x: T] *)
+| ty_var_p : forall G x T,
+    binds x T G ->
+    G ⊢! trm_var (avar_f x) : T
+
+(** [G, x: T ⊢ t^x: U^x]       #<br>#
+    [x fresh]                  #<br>#
+    [――――――――――――――――――――――――] #<br>#
+    [G ⊢! lambda(T)t: forall(T) U]     *)
+| ty_all_intro_p : forall L G T t U,
+    (forall x, x \notin L ->
+      G & x ~ T ⊢ open_trm x t : open_typ x U) ->
+    G ⊢! trm_val (val_lambda T t) : typ_all T U
+
+(** [G, x: T^x ⊢ ds^x :: T^x]   #<br>#
+    [x fresh]                   #<br>#
+    [―――――――――――――――――――――――]   #<br>#
+    [G ⊢! nu(T)ds :: mu(T)]        *)
+| ty_new_intro_p : forall L G T ds,
+    (forall x, x \notin L ->
+      G & (x ~ open_typ x T) /- open_defs x ds :: open_typ x T) ->
+    G ⊢! trm_val (val_new T ds) : typ_bnd T
+
+(** [G ⊢! x: mu(T)] #<br>#
+    [――――――――――――――] #<br>#
+    [G ⊢! x: T^x]       *)
+| ty_rec_elim_p : forall G x T,
+    G ⊢! trm_var (avar_f x) : typ_bnd T ->
+    G ⊢! trm_var (avar_f x) : open_typ x T
+
+(** [G ⊢! x: T /\ U] #<br>#
+    [――――――――――――――] #<br>#
+    [G ⊢! x: T]     *)
+| ty_and1_p : forall G x T U,
+    G ⊢! trm_var (avar_f x) : typ_and T U ->
+    G ⊢! trm_var (avar_f x) : T
+
+(** [G ⊢! x: T /\ U] #<br>#
+    [――――――――――――――] #<br>#
+    [G ⊢! x: U]     *)
+| ty_and2_p : forall G x T U,
+    G ⊢! trm_var (avar_f x) : typ_and T U ->
+    G ⊢! trm_var (avar_f x) : U
+where "G '⊢!' t ':' T" := (ty_trm_p G t T).
+
+Hint Constructors ty_trm_p.
+
+(** * Precise Flow *)
+(** We use the precise flow relation to reason about the relations between
+    the precise type of a variable [G ⊢! x: T] and the type that the variable
+    is bound to in the context [G(x)=T'].#<br>#
+    If [G(x) = T], the [precise_flow] relation describes all the types [U] that [x] can
+    derive through precise typing ([⊢!], see [ty_trm_p]).
+    If [precise_flow x G T U], then [G(x) = T] and [G ⊢! x: U].   #<br>#
+    For example, if [G(x) = mu(x: {a: T} /\ {B: S..U})], then we can derive the following
+    precise flows for [x]:                                                 #<br>#
+    [precise_flow x G mu(x: {a: T} /\ {B: S..U}) mu(x: {a: T} /\ {B: S..U}]  #<br>#
+    [precise_flow x G mu(x: {a: T} /\ {B: S..U}) {a: T} /\ {B: S..U}]        #<br>#
+    [precise_flow x G mu(x: {a: T} /\ {B: S..U}) {a: T}]                    #<br>#
+    [precise_flow x G mu(x: {a: T} /\ {B: S..U}) {B: S..U}]. *)
+Inductive precise_flow : var -> ctx -> typ -> typ -> Prop :=
+  | pf_bind : forall x G T,
+      binds x T G ->
+      precise_flow x G T T
+  | pf_open : forall x G T U,
+      precise_flow x G T (typ_bnd U) ->
+      precise_flow x G T (open_typ x U)
+  | pf_and1 : forall x G T U1 U2,
+      precise_flow x G T (typ_and U1 U2) ->
+      precise_flow x G T U1
+  | pf_and2 : forall x G T U1 U2,
+      precise_flow x G T (typ_and U1 U2) ->
+      precise_flow x G T U2.
+
+Hint Constructors precise_flow.
+
+
+(** If [precise_flow x G T U] then [G(x) = T]. *)
+Lemma pf_binds: forall G x T U,
+    precise_flow x G T U ->
+    binds x T G.
+Proof.
+  introv Pf. dependent induction Pf; auto.
+Qed.
+
+(** Introduces [precise_flow], given a variable's precise type. *)
+Lemma precise_flow_lemma : forall U G x,
+    G ⊢! trm_var (avar_f x) : U ->
+    exists T, precise_flow x G T U.
+Proof.
+  introv H. dependent induction H; try (destruct* (IHty_trm _ eq_refl));
+              try (destruct* (IHty_trm_p _ eq_refl)); eauto.
+Qed.
+
+(** If [G(x) = forall(S)T], then [x]'s precise type can be only [forall(S)T]. *)
+Lemma precise_flow_all_inv : forall p G S T U,
+    precise_flow p G (typ_all S T) U ->
+    U = typ_all S T.
+Proof.
+  introv Hpf.
+  dependent induction Hpf; auto;
+    specialize (IHHpf S T eq_refl); inversion IHHpf.
+Qed.
+
+(** The precise type of a value is inert. *)
+Lemma precise_inert_typ : forall G v T,
+    G ⊢! trm_val v : T ->
+    inert_typ T.
+Proof.
+  introv Ht. inversions Ht; constructor; rename T0 into T.
+  pick_fresh z. assert (Hz: z \notin L) by auto. specialize (H1 z Hz).
+  pose proof (ty_defs_record_type H1).
+  assert (Hz': z \notin fv_typ T) by auto.
+  apply (record_type_open T Hz' H).
+Qed.
+
+(** The following two lemmas say that the type to which a variable is bound in an inert context is inert. *)
+Lemma binds_inert : forall G x T,
+    binds x T G ->
+    inert G ->
+    inert_typ T.
+Proof.
+  introv Bi Hinert. induction Hinert.
+  - false * binds_empty_inv.
+  - destruct (binds_push_inv Bi).
+    + destruct H1. subst. assumption.
+    + destruct H1. apply (IHHinert H2).
+Qed.
+
+(** See [binds_inert]. *)
+Lemma pf_inert_T : forall G p T U,
+    inert G ->
+    precise_flow p G T U ->
+    inert_typ T.
+Proof.
+  introv Hi Pf. induction Pf; eauto.
+  apply (binds_inert H Hi).
+Qed.
+
+(** See [inert_typ_bnd_record] *)
+Lemma pf_rcd_T : forall G p T U,
+    inert G ->
+    precise_flow p G (typ_bnd T) U ->
+    record_type T.
+Proof.
+  introv Hi Pf. apply pf_inert_T in Pf; inversions Pf; assumption.
+Qed.
+
+(** If [G(x) = mu(x: T)], then [x]'s precise type can be only [mu(x: T)]
+     or a record type. *)
+Lemma pf_inert_or_rcd : forall G x T U,
+    inert G ->
+    precise_flow x G (typ_bnd T) U ->
+    U = typ_bnd T \/ record_type U.
+Proof.
+  introv Hi Pf.
+  dependent induction Pf; try solve [left*].
+  - specialize (IHPf T Hi eq_refl). destruct IHPf as [eq | r].
+    * inversions eq. right. lets Hr: (pf_rcd_T Hi Pf).
+      apply* open_record_type.
+    * inversion r. inversion H.
+  - right. destruct (IHPf T Hi eq_refl) as [F | Hr]. inversion F.
+    inversion Hr. inversions H.
+    exists ls. assumption.
+  - right. destruct (IHPf T Hi eq_refl) as [F | Hr]. inversion F.
+    inversion Hr. inversions H.
+    eexists. apply* rt_one.
+Qed.
+
+(** If [x]'s precise type is [mu(x: U)], then [G(x) = mu(x: U)] *)
+Lemma pf_inert_bnd_U: forall G x T U,
+    inert G ->
+    precise_flow x G T (typ_bnd U) ->
+    T = typ_bnd U.
+Proof.
+  introv Hi Pf.
+  lets HT: (pf_inert_T Hi Pf).
+  inversions HT; dependent induction Pf; auto;
+    try (solve [apply pf_top_top in Pf; inversion Pf]).
+  - destruct U0; inversions x.
+    apply precise_flow_all_inv in Pf. inversion* Pf.
+  - apply precise_flow_all_inv in Pf. inversion Pf.
+  - apply precise_flow_all_inv in Pf. inversion Pf.
+  - specialize (IHPf U0 Hi T0 eq_refl eq_refl H).
+    destruct (pf_inert_or_rcd Hi Pf) as [Heq | Hr].
+    * inversions Heq. destruct T0; inversions x. inversion H. inversion H0.
+    * inversions IHPf. inversion Hr. inversions H0.
+  - destruct (pf_inert_or_rcd Hi Pf) as [Heq | Hr].
+    * inversions Heq.
+    * inversions Hr. inversions H0. inversions H3.
+  - destruct (pf_inert_or_rcd Hi Pf) as [Heq | Hr].
+    * inversions Heq.
+    * inversions Hr. inversions H0.
+Qed.
+
+(** If [x]'s precise type is a field or type declaration, then [G(x)] is
+    a recursive type. *)
+Lemma pf_inert_rcd_U: forall G x T D,
+    inert G ->
+    precise_flow x G T (typ_rcd D) ->
+    exists U, T = typ_bnd U.
+Proof.
+  introv Hi Pf.
+  lets HT: (pf_inert_T Hi Pf).
+  inversions HT; dependent induction Pf; auto;
+    try (solve [apply pf_top_top in Pf; inversion Pf]).
+  - apply precise_flow_all_inv in Pf. inversion Pf.
+  - apply precise_flow_all_inv in Pf. inversion Pf.
+  - apply precise_flow_all_inv in Pf. inversion Pf.
+  - apply (pf_inert_bnd_U Hi) in Pf. exists* U.
+  - exists* T0.
+  - exists* T0.
+Qed.
+
+
+(** If [x]'s precise type is a record type, then [G(x)] is a recursive type. *)
+Lemma pf_inert_rcd_typ_U: forall G x T Ds,
+    inert G ->
+    precise_flow x G T Ds ->
+    record_type Ds ->
+    exists U, T = typ_bnd U.
+Proof.
+  introv Hi Pf Hr.
+  lets HT: (pf_inert_T Hi Pf).
+  inversions HT;
+    try (solve [apply pf_top_top in Pf; subst;
+                unfold record_type in *;
+                destruct Hr; remember typ_top; destruct H; inversion Heqt]);
+    dependent induction Pf; auto.
+  - inversion Hr. inversion H0.
+  - apply precise_flow_all_inv in Pf. inversion Pf.
+  - apply precise_flow_all_inv in Pf. inversion Pf.
+  - apply precise_flow_all_inv in Pf. inversion Pf.
+  - inversion Hr. inversion H1.
+  - apply (pf_inert_bnd_U Hi) in Pf. exists* U.
+  - apply* IHPf. destruct (pf_inert_or_rcd Hi Pf) as [H1 | H1].
+    inversion H1. assumption.
+  - apply* IHPf. destruct (pf_inert_or_rcd Hi Pf) as [H1 | H1].
+    inversion H1. assumption.
+Qed.
+
+(** The following two lemmas express that if [x]'s precise type is a function type,
+    then [G(x)] is the same function type. *)
+Lemma pf_inert_lambda_U : forall x G S T U,
+    inert G ->
+    precise_flow x G U (typ_all S T) ->
+    U = typ_all S T.
+Proof.
+  introv Hi Pf.
+  lets Hiu: (pf_inert_T Hi Pf).
+  inversions Hiu.
+  - apply precise_flow_all_inv in Pf. inversion* Pf.
+  - destruct (pf_inert_or_rcd Hi Pf) as [H1 | H1]; inversions H1.
+    inversion H0.
+Qed.
+
+(** See [pf_inert_lambda_U]. *)
+Lemma inert_precise_all_inv : forall x G S T,
+    inert G ->
+    G ⊢! trm_var (avar_f x) : typ_all S T ->
+    binds x (typ_all S T) G.
+Proof.
+  introv Hgd Htyp.
+  destruct (precise_flow_lemma Htyp) as [V Pf].
+  pose proof (pf_inert_lambda_U Hgd Pf) as H. subst.
+  apply* pf_binds.
+Qed.
+
+(** The following two lemmas say that in an inert context, the precise type of a variable
+    cannot be bottom. *)
+Lemma pf_bot_false : forall G x T,
+    inert G ->
+    precise_flow x G T typ_bot ->
+    False.
+Proof.
+  introv Hi Pf.
+  lets HT: (pf_inert_T Hi Pf). inversions HT.
+  - apply precise_flow_all_inv in Pf. inversion Pf.
+  - destruct (pf_inert_or_rcd Hi Pf); inversion H0. inversion H1.
+Qed.
+
+(** See [pf_bot_false]. *)
+Lemma precise_bot_false : forall G x,
+    inert G ->
+    G ⊢! trm_var (avar_f x) : typ_bot ->
+    False.
+Proof.
+  introv Hi Hp. destruct (precise_flow_lemma Hp) as [T Pf].
+  apply* pf_bot_false.
+Qed.
+
+(** The following two lemmas say that in an inert context, the precise type of
+    a variable cannot be type selection. *)
+Lemma pf_psel_false : forall G T x y A,
+    inert G ->
+    precise_flow x G T (typ_sel y A) ->
+    False.
+Proof.
+  introv Hi Pf.
+  lets HT: (pf_inert_T Hi Pf). inversions HT.
+  - apply precise_flow_all_inv in Pf. inversion Pf.
+  - destruct (pf_inert_or_rcd Hi Pf); inversion H0. inversion H1.
+Qed.
+
+(** See [pf_psel_false]. *)
+Lemma precise_psel_false : forall G x y A,
+    inert G ->
+    G ⊢! trm_var (avar_f x) : typ_sel y A ->
+    False.
+Proof.
+  introv Hi Hp. destruct (precise_flow_lemma Hp) as [T Pf].
+  apply* pf_psel_false.
+Qed.
+
+(** If [G(x) = mu(T)], and [G ⊢! x: ... /\ D /\ ...], then [T^x = ... /\ D /\ ...]. *)
+Lemma pf_record_sub : forall x G T T' D,
+    inert G ->
+    precise_flow x G (typ_bnd T) T' ->
+    record_has T' D ->
+    record_has (open_typ x T) D.
+Proof.
+  introv Hi Pf Hr. dependent induction Pf.
+  - inversions Hr.
+  - apply (pf_inert_bnd_U Hi) in Pf. inversion* Pf.
+  - apply* IHPf.
+  - apply* IHPf.
+Qed.
+
+(** If [G(x) = mu(S)] and [G ⊢! x: D], where [D] is a field or type declaration,
+    then [S^x = ... /\ D /\ ...]. *)
+Lemma precise_flow_record_has: forall S G x D,
+    inert G ->
+    precise_flow x G (typ_bnd S) (typ_rcd D) ->
+    record_has (open_typ x S) D.
+Proof.
+  introv Hi Pf. apply* pf_record_sub.
+Qed.
+
+(** If
+    - [G(x) = mu(T)]
+    - [G ⊢! x: {A: T1..T1}]
+    - [G ⊢! x: {A: T2..T2}]
+    then [T1 = T2]. *)
+Lemma pf_record_unique_tight_bounds_rec : forall G x T A T1 T2,
+    inert G ->
+    precise_flow x G (typ_bnd T) (typ_rcd (dec_typ A T1 T1)) ->
+    precise_flow x G (typ_bnd T) (typ_rcd (dec_typ A T2 T2)) ->
+    T1 = T2.
+Proof.
+  introv Hi Pf1 Pf2.
+  pose proof (precise_flow_record_has Hi Pf1) as H1.
+  pose proof (precise_flow_record_has Hi Pf2) as H2.
+  eapply unique_rcd_typ; eauto. apply (pf_rcd_T Hi) in Pf1.
+  apply* open_record_type.
+Qed.
+
+(** If
+    - [G ⊢! x: {A: T1..T1}]
+    - [G ⊢! x: {A: T2..T2}]
+    then [T1 = T2]. *)(** *)
+Lemma pf_inert_unique_tight_bounds : forall G x T T1 T2 A,
+    inert G ->
+    precise_flow x G T (typ_rcd (dec_typ A T1 T1)) ->
+    precise_flow x G T (typ_rcd (dec_typ A T2 T2)) ->
+    T1 = T2.
+Proof.
+  introv Hi Pf1 Pf2.
+  assert (record_type (typ_rcd (dec_typ A T1 T1))) as Hrt. {
+    unfold record_type. eexists. apply* rt_one.
+    constructor.
+  }
+  lets Hr: (pf_inert_rcd_typ_U Hi Pf1 Hrt). destruct Hr as [U Heq]. subst.
+  apply* pf_record_unique_tight_bounds_rec.
+Qed.
+
+(** The type to which a variable is bound in an environment is unique. *)
+Lemma x_bound_unique: forall G x T1 T2 U1 U2,
+    inert G ->
+    precise_flow x G T1 U1 ->
+    precise_flow x G T2 U2 ->
+    T1 = T2.
+Proof.
+  introv Hi Pf1. gen T2 U2. induction Pf1; intros;
+                              try solve [apply* IHPf1]; auto.
+  apply pf_binds in H0. apply (binds_func H H0).
+Qed.
+
+(** See [pf_inert_unique_tight_bound]. *)
+Lemma inert_unique_tight_bounds : forall G x T1 T2 A,
+    inert G ->
+    G ⊢! trm_var (avar_f x) : typ_rcd (dec_typ A T1 T1) ->
+    G ⊢! trm_var (avar_f x) : typ_rcd (dec_typ A T2 T2) ->
+    T1 = T2.
+Proof.
+  introv Hi H1 H2.
+  destruct (precise_flow_lemma H1) as [T1' Pf1].
+  destruct (precise_flow_lemma H2) as [T2' Pf2].
+  lets Heq: (x_bound_unique Hi Pf1 Pf2). subst.
+  apply* pf_inert_unique_tight_bounds.
+Qed.
+
+(** If a typing context is inert, then the variables in its domain are distinct. #<br>#
+    Note: [ok] is defined in [TLC.LibEnv.v]. *)
+Lemma inert_ok : forall G,
+    inert G ->
+    ok G.
+Proof.
+  intros G HG. induction G using env_ind.
+  auto.
+  inversions HG. false* empty_push_inv.
+  destruct (eq_push_inv H) as [Hx [HT HG]]. subst.
+  apply* ok_push.
+Qed.
+
+Hint Resolve inert_ok.
+
+(** The following two lemmas express that if [G ⊢! x: {A: S..U}] then [S = U]. *)
+Lemma pf_dec_typ_inv : forall G x T A S U,
+    inert G ->
+    precise_flow x G T (typ_rcd (dec_typ A S U)) ->
+    S = U.
+Proof.
+  introv Hi Pf. destruct (pf_inert_rcd_U Hi Pf) as [V H]. subst.
+  destruct (pf_inert_or_rcd Hi Pf) as [H1 | H1]; inversions H1. inversions H.
+  inversions* H1.
+Qed.
+
+(** See [pf_dec_typ_inv]. *)
+Lemma precise_dec_typ_inv : forall G x A S U,
+    inert G ->
+    G ⊢! trm_var (avar_f x) : typ_rcd (dec_typ A S U) ->
+    S = U.
+Proof.
+  introv Hi Hpt. destruct (precise_flow_lemma Hpt) as [V Pf].
+  apply* pf_dec_typ_inv.
+Qed.
+
+(** Precise typing implies general typing. *)
+Lemma precise_to_general: forall G t T,
+    G ⊢! t : T ->
+    G ⊢ t : T.
+Proof.
+  intros. induction H; intros; subst; eauto.
+Qed.
