src/simple-proof/proof-stacks/Safety.v
@@ -1,0 +1,171 @@
+Set Implicit Arguments.
+
+Require Import LibLN.
+Require Import Coq.Program.Equality.
+Require Import Definitions Weakening Narrowing Binding PreciseTypes Substitution CanonicalForms
+        RecordAndInertTypes InvertibleTypes GeneralToTight.
+
+Reserved Notation "s1 '//' t1 '|->' s2 '//' t2" (at level 40, s2 at level 39).
+
+Inductive ec_red : trm -> ec -> trm -> ec -> Prop :=
+| red_sel : forall x m e t T ds,
+    binds x (val_new T ds) e ->
+    defs_has (open_defs x ds) (def_trm m t) ->
+    e // trm_sel (avar_f x) m |-> e // t
+| red_app : forall f a e T t,
+    binds f (val_lambda T t) e ->
+    e // trm_app (avar_f f) (avar_f a) |-> e // open_trm a t
+| red_let : forall v t s x,
+    x # s ->
+    s // trm_let (trm_val v) t |-> s & x ~ v // open_trm x t
+| red_let_var : forall t e x,
+    e // trm_let (trm_var (avar_f x)) t |-> e // open_trm x t
+| red_let_tgt : forall t0 t e t0' e',
+    e // t0 |-> e' // t0' ->
+    e // trm_let t0 t |-> e' // trm_let t0' t
+where "e1 // t1 |-> e2 // t2" := (ec_red t1 e1 t2 e2).
+
+Inductive sto_trm_typ : ec -> trm -> typ -> Prop :=
+| sto_trm_typ_c : forall G e t T,
+    inert G ->
+    well_typed G e ->
+    G ⊢ t : T ->
+    sto_trm_typ e t T.
+
+Notation "'⊢' e ',' t ':' T" := (sto_trm_typ e t T) (at level 40, t at level 59).
+
+Inductive norm_form: trm -> Prop :=
+| nf_var: forall x, norm_form (trm_var x)
+| nf_val: forall v, norm_form (trm_val v).
+
+Hint Constructors norm_form.
+
+(** If a value [v] has type [T], then [v] has a precise type [T']
+    that is a subtype of [T].
+    This lemma corresponds to Lemma 3.15 in the paper. *)
+Lemma val_typing: forall G v T,
+  G ⊢ trm_val v : T ->
+  exists T', G ⊢! trm_val v : T' /\
+        G ⊢ T' <: T.
+Proof.
+  intros G v T H. dependent induction H; eauto.
+  destruct (IHty_trm _ eq_refl) as [T' [Hty Hsub]]. eauto.
+Qed.
+
+Lemma preservation_ty: forall G e t e' t' T,
+    well_typed G e ->
+    inert G ->
+    e // t |-> e' // t' ->
+    G ⊢ t : T ->
+    exists G', inert G' /\
+          well_typed (G & G') e' /\
+          G & G' ⊢ t' : T.
+Proof.
+  introv Hwf Hin Hred Ht.
+  gen t'.
+  dependent induction Ht; intros; try solve [inversions Hred].
+  - pose proof (canonical_forms_fun Hin Hwf Ht1) as [L [T' [t [Bis [Hsub Hty]]]]].
+    inversions Hred.
+    apply (binds_func H4) in Bis. inversions Bis.
+    exists (@empty typ). rewrite concat_empty_r. repeat split; auto.
+    pick_fresh y. assert (y \notin L) as FrL by auto. specialize (Hty y FrL).
+    rewrite subst_intro_typ with (x:=y); auto.
+    rewrite subst_intro_trm with (x:=y); auto.
+    eapply subst_ty_trm; eauto. rewrite~ subst_fresh_typ.
+  - pose proof (canonical_forms_obj Hin Hwf Ht) as [S [ds [t [Bis [Has Ty]]]]].
+    inversions Hred.
+    apply (binds_func H1) in Bis. inversions Bis.
+    exists (@empty typ). rewrite concat_empty_r. repeat split; auto.
+    rewrite <- (defs_has_inv Has H5). assumption.
+  - destruct t.
+    + inversions Hred; try solve [inversion H6].
+      pick_fresh y.
+      exists (@empty typ). rewrite concat_empty_r. repeat split; auto.
+      rewrite subst_intro_trm with (x:=y); auto.
+      rewrite <- subst_fresh_typ with (x:=y) (y:=x); auto.
+      eapply subst_ty_trm; eauto. rewrite~ subst_fresh_typ.
+    + inversions Hred; try solve [inversion H6].
+      pose proof (well_typed_notin_dom Hwf H6).
+      pose proof (val_typing Ht) as [V [Hv Hs]].
+      pick_fresh y. assert (y \notin L) by auto.
+      specialize (H y H2).
+      exists (x ~ V). repeat split.
+      * rewrite <- concat_empty_l. constructor~.
+        apply (precise_inert_typ Hv).
+      * constructor~.
+        apply (precise_to_general Hv).
+      * rewrite subst_intro_trm with (x:=y); auto.
+        rewrite <- subst_fresh_typ with (x:=y) (y:=x); auto.
+        eapply subst_ty_trm; eauto.
+        { eapply weaken_rules; eauto. }
+        { apply~ fv_ctx_types_push. }
+        { rewrite~ subst_fresh_typ.
+          pose proof (ty_var (binds_tail x V G)).
+          apply (ty_sub H3). apply (weaken_subtyp Hs); eauto.
+        }
+    + inversions Hred.
+      specialize (IHHt Hwf Hin t0' H6) as [G' [Hin' [Hwf' Ht']]].
+      exists G'. repeat split; auto.
+      apply_fresh ty_let as z; eauto.
+      eapply weaken_rules; eauto.
+    + inversions Hred.
+      specialize (IHHt Hwf Hin t0' H6) as [G' [Hin' [Hwf' Ht']]].
+      exists G'. repeat split; auto.
+      apply_fresh ty_let as z; eauto.
+      eapply weaken_rules; eauto.
+    + inversions Hred.
+      specialize (IHHt Hwf Hin t0' H6) as [G' [Hin' [Hwf' Ht']]].
+      exists G'. repeat split; auto.
+      apply_fresh ty_let as z; eauto.
+      eapply weaken_rules; eauto.
+  - specialize (IHHt Hwf Hin t' Hred) as [G' [Hin' [Hwf' Ht']]].
+    exists G'. repeat split; auto.
+    apply weaken_subtyp with (G2:=G') in H.
+    + apply (ty_sub Ht' H).
+    + eauto.
+Qed.
+
+Theorem preservation : forall e e' t t' T,
+    ⊢ e, t : T ->
+    e // t |-> e' // t' ->
+    ⊢ e', t' : T.
+Proof.
+  introv Ht Hr. destruct Ht as [* Hi Hwf Ht].
+  lets Hp: (preservation_ty Hwf Hi Hr Ht). destruct Hp as [G' [Hi' [Hwf' Ht']]].
+  apply sto_trm_typ_c with (G:=G&G'); auto. apply* inert_concat.
+Qed.
+
+Theorem progress: forall e t T,
+    ⊢ e, t : T ->
+    norm_form t \/ exists e' t', e // t |-> e' // t'.
+Proof.
+  introv Ht. destruct Ht as [* Hin Hwf Ht].
+  induction Ht; try solve [left; auto].
+  - pose proof (canonical_forms_fun Hin Hwf Ht1) as [L [T' [t [Bis [Hsub Hty]]]]].
+    right. exists e (open_trm z t).
+    eapply red_app; eauto.
+  - pose proof (canonical_forms_obj Hin Hwf Ht) as [S [ds [t [Bis [Has Ty]]]]].
+    right. exists e t.
+    eapply red_sel; eauto.
+  - right. destruct t.
+    + pose proof (var_typing_implies_avar_f Ht) as [x A]. subst.
+      exists e (open_trm x u). apply red_let_var.
+    + pick_fresh x.
+      exists (e & x ~ v) (open_trm x u).
+      eapply red_let; auto.
+    + specialize (IHHt Hin Hwf) as [IH | [e' [t' Hred]]].
+      * inversion IH.
+      * exists e' (trm_let t' u).
+        apply~ red_let_tgt.
+    + specialize (IHHt Hin Hwf) as [IH | [e' [t' Hred]]].
+      * inversion IH.
+      * exists e' (trm_let t' u).
+        apply~ red_let_tgt.
+    + specialize (IHHt Hin Hwf) as [IH | [e' [t' Hred]]].
+      * inversion IH.
+      * exists e' (trm_let t' u).
+        apply~ red_let_tgt.
+  - specialize (IHHt Hin Hwf) as [IH | [e' [t' Hred]]].
+    + left. assumption.
+    + right. exists e' t'. assumption.
+Qed.
